proved monad transformer laws for option_t using generic equality framework. big step forward.  currently struggling with adding new Proper proofs that are based on generic equality, and using them in a setting with specific equality.  Also encoutering the problem where ideally deriving should derive abstrct equality based on underlying abstract equality.  This could work out, but now we must do the same for ord, lattice, etc.  Do I really want equivalence environments to creep in everywhere in the library?  _probably not_.  Currently going to _back peddle_ and get rid of abstract equality, and settle on everything being proved directly against the Eqv typeclass.  This may or may not work out.  If it doesn't, come back to this snapshot, because I'm going to start aggressively ripping out EqvEnv and generic abstract equality.

src/Data/Option.v
@@ -3,7 +3,9 @@ Require Import FP.Data.Function.
 Require Import FP.Data.Identity.
 Require Import FP.Data.Sum.
 Require Import FP.Data.Unit.
+Require Import FP.Data.SumRelations.
 Require Import FP.Structures.Additive.
+Require Import FP.Structures.EqvEnv.
 Require Import FP.Structures.Comonad.
 Require Import FP.Structures.EqDec.
 Require Import FP.Structures.Eqv.
@@ -12,12 +14,14 @@ Require Import FP.Structures.Lattice.
 Require Import FP.Structures.Functor.
 Require Import FP.Structures.Functor.
 Require Import FP.Structures.Monad.
+Require Import FP.Structures.Applicative.
 Require Import FP.Structures.Counit.
 Require Import FP.Structures.Injection.
 Require Import FP.Structures.FUnit.
 Require Import FP.Structures.Injection.
 Require Import FP.Structures.Monad.
 Require Import FP.Structures.MonadError.
+Require Import FP.Structures.Proxy.
 Require Import FP.Structures.Deriving.
 Require Import FP.Structures.FUnit.
 Require Import FP.Structures.FUnitDeriving.
@@ -52,9 +56,10 @@ Section sum_Bijection.
     end.
   Global Instance option_to_sum_InjectionResp_eq
       : InjectionRespect (option A) (unit+A) option_to_sum eq eq.
+  Proof.
     constructor ; unfold Proper ; simpl in * ; intros ; try congruence.
     destruct x,y ; simpl in * ; congruence.
-    Qed.
+  Qed.
 
   Definition sum_to_option (aM:unit+A) : option A :=
     match aM with
@@ -63,9 +68,10 @@ Section sum_Bijection.
     end.
   Global Instance sum_to_option_InjectionInverse_eq
       : InjectionInverse (unit+A) (option A) sum_to_option option_to_sum eq.
+  Proof.
     constructor ; intros.
     destruct x ; [ destruct u | idtac ] ; simpl in * ; auto.
-    Qed.
+  Qed.
 End sum_Bijection.
 
 Module option_DTKS1_Arg <: DerivingTheKitchenSink1_Arg.
@@ -75,10 +81,119 @@ Module option_DTKS1_Arg <: DerivingTheKitchenSink1_Arg.
   Definition from {A} (x:U A) := sum_to_option x.
   Definition InjResp A : InjectionRespect (T A) (U A) to eq eq := _.
   Definition InjInv A : InjectionInverse (U A) (T A) from to eq := _.
+  Definition U_EqDec :
+    forall {A} {EqDec_:EqDec A},
+    EqDec (U A) := _.
+  Definition U_EqDec_RDC :
+    forall {A} {EqDec_:EqDec A} {EqDec_RDC:RelDecCorrect A eq eq_dec},
+    RelDecCorrect (U A) eq eq_dec := _.
+  Definition U_Eqv :
+    forall {A} {Eqv_:Eqv A},
+    Eqv (U A) := _.
+  Definition U_Eqv_PE_WF :
+    forall {A} {Eqv_:Eqv A} {Eqv_PE_WF_:Eqv_PE_WF A},
+    Eqv_PE_WF (U A) := _.
+  Definition U_Eqv_E_WF :
+    forall {A} {Eqv_:Eqv A} {Eqv_PE_WF_:Eqv_E_WF A},
+    Eqv_E_WF (U A) := _.
+  Definition U_EqvDec :
+    forall {A} {EqvDec_:EqvDec A},
+    EqvDec (U A) := _.
+  Definition U_EqvDec_RDC :
+    forall {A} {Eqv_:Eqv A} {EqvDec_:EqvDec A} {EqvDec_RDC_:RelDecCorrect A eqv eqv_dec},
+    RelDecCorrect (U A) eqv eqv_dec := _.
+  Definition U_Ord :
+    forall {A} {Ord_:Ord A},
+    Ord (U A) := _.
+  Definition U_OrdWF :
+    forall {A} {Eqv_:Eqv A} {Eqv_E_WF_:Eqv_E_WF A} {Ord_:Ord A} {OrdWF_:OrdWF A},
+    OrdWF (U A) := _.
+  Definition U_OrdDec :
+    forall {A} {OrdDec_:OrdDec A},
+    OrdDec (U A) := _.
+  Definition U_ODC :
+    forall {A} {Eqv_:Eqv A} {Ord_:Ord A} {OrdDec_:OrdDec A} {ODC_:OrdDecCorrect A},
+    OrdDecCorrect (U A) := _.
+  Definition U_Lattice :
+    forall {A} {Lattice_:Lattice A},
+    Lattice (U A) := _.
+  Definition U_LatticeWF :
+    forall {A}
+      {Eqv_:Eqv A} {Eqv_E_WF_:Eqv_E_WF A}
+      {Ord_:Ord A} {OrdWF_:OrdWF A}
+      {Lattice_:Lattice A} {LatticeWF_:LatticeWF A},
+    LatticeWF (U A) := _.
+  Definition U_BoundedLattice :
+    forall {A} {BoundedLattice_:BoundedLattice A},
+    BoundedLattice (U A) := _.
+  Definition U_BoundedLatticeWF :
+    forall {A}
+      {Eqv_:Eqv A} {Eqv_E_WF_:Eqv_E_WF A}
+      {Ord_:Ord A} {OrdWF_:OrdWF A}
+      {Lattice_:Lattice A} {LatticeWF_:LatticeWF A}
+      {BoundedLattice_:BoundedLattice A} {BoundedLatticeWF_:BoundedLatticeWF A},
+    BoundedLatticeWF (U A) := _.
 End option_DTKS1_Arg.
 
 Module option_DTKS1 := DerivingTheKitchenSink1 option_DTKS1_Arg.
 Import option_DTKS1.
+
+Instance Some_InjectionRespect_eqv {A} {Eqv_:Eqv A} :
+  InjectionRespect A (option A) Some eqv eqv.
+Proof.
+  constructor ; unfold Proper,"==>","<==" ; intros.
+  constructor ; auto.
+  inversion H ; auto.
+Qed.
+
+Instance None_Proper {A} {Eqv_:Eqv A} :
+  Proper eqv (None (A:=A)).
+Proof.
+  unfold Proper,eqv ; simpl.
+  eapply InjectionRespect_eta ; reflexivity.
+Qed.
+
+Instance Some_Proper {A} {Eqv_:Eqv A} :
+  Proper eqv (Some (A:=A)).
+Proof.
+  apply eqv_env_logical_intro_eqv.
+  apply InjectionRespect_eta.
+Qed.
+
+Ltac destruct_option_eqv x y :=
+  match goal with
+  | [ e : eqv x y |- _ ] =>
+      destruct x,y ;
+      [ apply InjectionRespect_beta in e
+      | inversion e
+      | inversion e
+      | idtac ]
+  end.
+
+Definition option_elim {A C} (aM:option A) (z:C) (f:A -> C) : C :=
+  match aM with
+  | None => z
+  | Some a => f a
+  end.
+
+Global Instance option_elim_respect {A C} {aP:Eqv A} {cP:Eqv C} :
+  Proper eqv (option_elim (A:=A) (C:=C)).
+Proof.
+  unfold option_elim.
+  logical_eqv_eqv.
+  destruct_option_eqv x y ; logical_eqv_eqv.
+Qed.
+
+Ltac fold_option_elim :=
+  match goal with
+  | [ |- context
+         [ match ?aM with
+           | None => ?z
+           | Some a => (@?f a)
+           end
+         ]
+    ] => fold (option_elim aM z f)
+  end.
 
 Definition from_option {A} (a:A) (aM:option A) : A :=
   match aM with
@@ -95,18 +210,6 @@ Section throw_msg_option.
     | Some x => ret x
     end.
 End throw_msg_option.
-
-(*
-Section zero_option.
-  Context {m} {M:Monad m} {P:MonadPlus m}.
-
-  Definition zero_option {A} (xM:option A) : m A :=
-    match xM with
-    | None => mzero
-    | Some x => ret x
-    end.
-End zero_option.
-*)
 
 Section monoid_option.
   Context {T} {TM:Monoid T}.
@@ -135,6 +238,251 @@ Inductive option_t m (A:Type) := OptionT { un_option_t : m (option A) }.
 Arguments OptionT {m A} _.
 Arguments un_option_t {m A} _.
 
+Section m_option_Bijection.
+  Context {m:Type -> Type} {A:Type}.
+
+  Definition option_t_to_m_option : option_t m A -> m (option A) := un_option_t.
+  Global Instance option_t_to_m_option_InjectionResp_eq
+      : InjectionRespect (option_t m A) (m (option A)) option_t_to_m_option eq eq.
+  Proof.
+    constructor ; try congruence.
+    unfold Proper,"<==" ; intros.
+    destruct x,y ; simpl in * ; congruence.
+  Qed.
+  Arguments option_t_to_m_option _ /.
+
+  Definition m_option_to_option_t : m (option A) -> option_t m A := OptionT.
+  Global Instance m_option__to_option_t_InjectionInverse_eq
+      : InjectionInverse (m (option A)) (option_t m A)
+                         m_option_to_option_t option_t_to_m_option eq.
+  Proof.
+    constructor ; auto.
+  Qed.
+End m_option_Bijection.
+
+Module option_t_DTKS2_Arg <: DerivingTheKitchenSink2_Arg.
+  Definition T (m:Type->Type) A := option_t m A.
+  Definition U (m:Type->Type) A := m (option A).
+  Definition to {m A} (x:T m A) := option_t_to_m_option x.
+  Definition from {m A} (x:U m A) := m_option_to_option_t x.
+  Definition InjResp m A : InjectionRespect (T m A) (U m A) to eq eq := _.
+  Definition InjInv m A : InjectionInverse (U m A) (T m A) from to eq := _.
+  Section m.
+    Context {m:Type->Type}.
+    Definition U_EqDec :
+      forall
+        {EqDec_m :
+           forall {X} {EqDec_:EqDec X},
+           EqDec (m X)}
+        {A} {EqDec_:EqDec A},
+      EqDec (U m A) := _.
+    Definition U_EqDec_RDC :
+      forall
+        {EqDec_m :
+           forall {X} {EqDec_:EqDec X},
+           EqDec (m X)}
+        {EqDec_RDC_m :
+           forall {X} {EqDec_:EqDec X} {EqDec_RDC_:RelDecCorrect X eq eq_dec},
+           RelDecCorrect (m X) eq eq_dec}
+        {A} {EqDec_:EqDec A} {RDC_A:RelDecCorrect A eq eq_dec},
+      RelDecCorrect (U m A) eq eq_dec := _.
+    Definition U_Eqv :
+      forall
+        {Eqv_m :
+           forall {X} {Eqv_:Eqv X},
+           Eqv (m X)}
+        {A} {Eqv_:Eqv A},
+      Eqv (U m A) := _.
+    Definition U_Eqv_PE_WF :
+      forall
+        {Eqv_m :
+           forall {X} {Eqv_:Eqv X},
+           Eqv (m X)}
+        {Eqv_PE_WF_m :
+           forall {X} {Eqv_:Eqv X} {Eqv_PE_WF_:Eqv_PE_WF X},
+           Eqv_PE_WF (m X)}
+        {A} {Eqv_:Eqv A} {Eqv_PE_WF_:Eqv_PE_WF A},
+      Eqv_PE_WF (U m A) := _.
+    Definition U_Eqv_E_WF :
+      forall
+        {Eqv_m :
+           forall {X} {Eqv_:Eqv X},
+           Eqv (m X)}
+        {Eqv_E_WF_m :
+           forall {X} {Eqv_:Eqv X} {Eqv_E_WF_:Eqv_E_WF X},
+           Eqv_E_WF (m X)}
+        {A} {Eqv_:Eqv A} {Eqv_E_WF_:Eqv_E_WF A},
+      Eqv_E_WF (U m A) := _.
+    Definition U_EqvDec :
+      forall
+        {EqvDec_m :
+           forall {X} {EqvDec_:EqvDec X},
+            EqvDec (m X)}
+        {A} {EqvDec_:EqvDec A},
+      EqvDec (U m A) := _.
+    Definition U_EqvDec_RDC :
+      forall
+        {Eqv_m :
+           forall {X} {Eqv_:Eqv X},
+           Eqv (m X)}
+        {EqvDec_m :
+           forall {X} {EqvDec_:EqvDec X},
+           EqvDec (m X)}
+        {EqvDec_RDC_m :
+           forall
+             {X} {Eqv_:Eqv X} {EqvDec_:EqvDec X}
+             {RDC_A:RelDecCorrect X eqv eqv_dec},
+           RelDecCorrect (m X) eqv eqv_dec}
+        {A} {Eqv_:Eqv A} {EqvDec_:EqvDec A} {RDC_A:RelDecCorrect A eqv eqv_dec},
+      RelDecCorrect (U m A) eqv eqv_dec := _.
+    Definition U_Ord :
+      forall
+        {Ord_m :
+           forall {X} {Ord_:Ord X},
+           Ord (m X)}
+        {A} {Ord_:Ord A},
+      Ord (U m A) := _.
+    Definition U_OrdWF :
+      forall
+        {Eqv_m :
+           forall {X} {Eqv_:Eqv X},
+           Eqv (m X)}
+        {Eqv_E_WF_m :
+           forall {X} {Eqv_:Eqv X} {Eqv_E_WF_:Eqv_E_WF X},
+           Eqv_E_WF (m X)}
+        {Ord_m :
+           forall {X} {Ord_:Ord X},
+           Ord (m X)}
+        {OrdWF_m :
+           forall
+             {X}
+             {Eqv_:Eqv X} {Eqv_E_WF_:Eqv_E_WF X}
+             {Ord_:Ord X} {Ord_WF_:OrdWF X},
+           OrdWF (m X)}
+        {A}
+        {Eqv_:Eqv A} {Eqv_E_WF_:Eqv_E_WF A}
+        {Ord_:Ord A} {Ord_WF_:OrdWF A},
+      OrdWF (U m A) := _.
+    Definition U_OrdDec :
+      forall
+        {OrdDec_m :
+           forall {X} {OrdDec_:OrdDec X},
+           OrdDec (m X)}
+        {A} {OrdDec_:OrdDec A},
+      OrdDec (U m A) := _.
+    Definition U_ODC :
+      forall
+        {Eqv_m :
+           forall {X} {Eqv_:Eqv X},
+           Eqv (m X)}
+        {Ord_m :
+           forall {X} {Ord_:Ord X},
+           Ord (m X)}
+        {OrdDec_m :
+           forall {X} {OrdDec_:OrdDec X},
+           OrdDec (m X)}
+        {ODC_m :
+           forall
+             {X} {Eqv_:Eqv X}
+             {Ord_:Ord X} {OrdDec_:OrdDec X} {ODC_A:OrdDecCorrect X},
+           OrdDecCorrect (m X)}
+        {A}
+        {Eqv_:Eqv A}
+        {Ord_:Ord A} {OrdDec_:OrdDec A} {ODC_A:OrdDecCorrect A},
+      OrdDecCorrect (U m A) := _.
+    Definition U_Lattice :
+      forall
+        {Lattice_m :
+           forall {X} {Lattice_:Lattice X},
+           Lattice (m X)}
+        {A} {Lattice_:Lattice A},
+      Lattice (U m A) := _.
+    Definition U_LatticeWF :
+      forall
+        {Eqv_m :
+           forall {X} {Eqv_:Eqv X},
+           Eqv (m X)}
+        {Eqv_E_WF_m :
+           forall {X} {Eqv_:Eqv X} {Eqv_E_WF_:Eqv_E_WF X},
+           Eqv_E_WF (m X)}
+        {Ord_m :
+           forall {X} {Ord_:Ord X},
+           Ord (m X)}
+        {OrdWF_m :
+           forall
+             {X}
+             {Eqv_:Eqv X} {Eqv_E_WF_:Eqv_E_WF X}
+             {Ord_:Ord X} {Ord_WF_:OrdWF X},
+           OrdWF (m X)}
+        {Lattice_m :
+           forall {X} {Lattice_:Lattice X},
+           Lattice (m X)}
+        {LatticeWF_m :
+           forall {X}
+             {Eqv_:Eqv X} {Eqv_E_WF_:Eqv_E_WF X}
+             {Ord_:Ord X} {OrdWF_:OrdWF X}
+             {Lattice_:Lattice X} {LatticeWF_:LatticeWF X},
+           LatticeWF (m X)}
+        {A}
+        {Eqv_:Eqv A} {Eqv_E_WF_:Eqv_E_WF A}
+        {Ord_:Ord A} {OrdWF_:OrdWF A}
+        {Lattice_:Lattice A} {LatticeWF_:LatticeWF A},
+      LatticeWF (U m A) := _.
+    Definition U_BoundedLattice :
+      forall 
+        {BoundedLattice_m :
+           forall {X} {BoundedLattice_:BoundedLattice X},
+           BoundedLattice (m X)}
+        {A} {BoundedLattice_:BoundedLattice A},
+      BoundedLattice (U m A) := _.
+    Definition U_BoundedLatticeWF :
+      forall
+        {Eqv_m :
+           forall {X} {Eqv_:Eqv X},
+           Eqv (m X)}
+        {Eqv_E_WF_m :
+           forall {X} {Eqv_:Eqv X} {Eqv_E_WF_:Eqv_E_WF X},
+           Eqv_E_WF (m X)}
+        {Ord_m :
+           forall {X} {Ord_:Ord X},
+           Ord (m X)}
+        {OrdWF_m :
+           forall
+             {X}
+             {Eqv_:Eqv X} {Eqv_E_WF_:Eqv_E_WF X}
+             {Ord_:Ord X} {Ord_WF_:OrdWF X},
+           OrdWF (m X)}
+        {Lattice_m :
+           forall {X} {Lattice_:Lattice X},
+           Lattice (m X)}
+        {LatticeWF_m :
+           forall {X}
+             {Eqv_:Eqv X} {Eqv_E_WF_:Eqv_E_WF X}
+             {Ord_:Ord X} {OrdWF_:OrdWF X}
+             {Lattice_:Lattice X} {LatticeWF_:LatticeWF X},
+           LatticeWF (m X)}
+        {BoundedLattice_m :
+           forall {X} {BoundedLattice_:BoundedLattice X},
+           BoundedLattice (m X)}
+        {BoundedLatticeWF_m :
+           forall {X}
+             {Eqv_:Eqv X} {Eqv_E_WF_:Eqv_E_WF X}
+             {Ord_:Ord X} {OrdWF_:OrdWF X}
+             {Lattice_:Lattice X} {LatticeWF_:LatticeWF X}
+             {BoundedLattice_:BoundedLattice X} {BoundedLatticeWF_:BoundedLatticeWF X},
+           BoundedLatticeWF (m X)}
+        {A}
+        {Eqv_:Eqv A} {Eqv_E_WF_:Eqv_E_WF A}
+        {Ord_:Ord A} {OrdWF_:OrdWF A}
+        {Lattice_:Lattice A} {LatticeWF_:LatticeWF A}
+        {BoundedLattice_:BoundedLattice A} {BoundedLatticeWF_:BoundedLatticeWF A},
+      BoundedLatticeWF (U m A) := _.
+  End m.
+End option_t_DTKS2_Arg.
+
+Module option_DTKS2 := DerivingTheKitchenSink2 option_t_DTKS2_Arg.
+Import option_DTKS2.
+
 Section MonadTrans.
   Definition option_t_lift {m} {M:Monad m} {A} : m A -> option_t m A :=
     OptionT '.' bind_fmap Some.
@@ -143,7 +491,7 @@ Section MonadTrans.
 End MonadTrans.
 
 Section option_t_Monad.
-  Context {m} {M:Monad m}.
+  Context {m} {FUnit_:FUnit m} {MBind_:MBind m}.
 
   Definition run_option_t {A} : option_t m A -> m (option A) := un_option_t.
 
@@ -165,7 +513,97 @@ Section option_t_Monad.
       { bind := @option_t_bind }.
   End Monad.
 
-  Global Instance option_t_FMap : FMap (option_t m) := Deriving_FMap_MBind.
+  Global Instance option_t_FApply : FApply (option_t m) := Deriving_FApply_MBind.
+  Global Instance option_t_FMap : FMap (option_t m) := Deriving_FMap_FApply.
+
+  Section MonadWF.
+    Local Instance EqvEnv_ : EqvEnv := eqv_EqvEnv.
+    Local Instance EqvEnvLogical_ : EqvEnvLogical := eqv_EqvEnvLogical.
+    Context {PE_R_m:forall {X} {aPER:Eqv X}, Eqv (m X)}.
+    Context {PE_R_m': forall {X} {aPER:Eqv X} {blah:Eqv_PE_WF X}, Eqv_PE_WF (m X)}.
+
+    Global Instance OptionT_respect {A} {aP:Eqv A} :
+      Proper eqv (OptionT (m:=m) (A:=A)).
+    Proof.
+      unfold Proper ; logical_eqv_intro_eqv ; auto.
+    Qed.
+
+    Global Instance un_option_t_respect {A} {aP:Eqv A} :
+      Proper eqv (un_option_t (m:=m) (A:=A)).
+    Proof.
+      unfold un_option_t ; simpl.
+      logical_eqv_eqv.
+    Qed.
+
+    Context {FUnitWF_:FUnitWF m}.
+
+    Global Instance option_t_FUnitWF : FUnitWF (option_t m).
+    Proof.
+      constructor ; intros.
+      unfold Proper,env_eqv,funit ; simpl.
+      logical_eqv_intro_eqv.
+      unfold eqv ; simpl ; logical_eqv_eqv.
+    Qed.
+    
+    Context {MonadWF_:MonadWF m}.
+
+    Global Instance option_t_MonadWF : MonadWF (option_t m).
+    Proof.
+      Local Ltac my_logical_eqv :=
+        repeat (try fold_option_elim ; logical_eqv_eqv).
+      constructor ; intros ;
+      unfold Proper,">>=",env_eqv ; simpl ; unfold "~=" ; simpl ;
+      unfold option_t_to_m_option.
+      - rewrite bind_left_unit_eqv ; my_logical_eqv.
+      - transitivity (un_option_t aM >>= funit) ; my_logical_eqv.
+        + destruct_option_eqv x y ; simpl ; my_logical_eqv.
+        + rewrite bind_right_unit_eqv ; my_logical_eqv.
+      - rewrite bind_associativity_eqv ; my_logical_eqv.
+        destruct_option_eqv x y ; simpl ; my_logical_eqv.
+        rewrite bind_left_unit_eqv ; my_logical_eqv.
+      - change (let (eqv) := Px_Eqv in eqv)
+        with (eqv (T:=option_t m A -> (A -> option_t m B) -> option_t m B)).
+        unfold option_t_bind ; my_logical_eqv.
+    Qed.
+
+    Global Instance option_t_MonadRespApplicative : MonadRespApplicative (option_t m).
+    Proof.
+      constructor ; intros.
+      change fapply with (bind_fapply (A:=A) (B:=B)).
+      logical_eqv.
+      assert (Proper env_eqv (bind_fapply (m:=option_t m) (A:=A) (B:=B))).
+      pose (bind_fapply_respect (m:=option_t m) (A:=A) (B:=B)).
+      Set Printing All.
+      Show.
+      simpl in p.
+      apply p.
+      Unset Printing All.
+      Show.
+      logical_eqv.
+      logical_eqv.
+      assert (P
+  End MonadWF.
+
+    Proof.
+      constructor ; intros.
+      change fapply with (bind_fapply (A:=A) (B:=B)).
+      eapply Proper_PE_R_app.
+      logical_eqv.
+      eapply bind_fapply_respect.
+      change env_eqv with (eqv (T:=option_t m B)).
+      logical_eqv_eqv.
+      eauto with typeclass_instances.
+      unfold bind_fapply.
+      logical_eqv.
+      unfold fapply. unfold option_t_FApply. unfold Deriving_FApply_MBind.
+      unfold deriving_FApply_MBind.
+      logical_eqv_eqv.
+      reflexivity.
+
+    Global Instance option_t_ApplicativeWF : ApplicativeWF (option_t m) :=
+        Deriving_ApplicativeWF_MonadWF.
+  End ApplicativeWF.
+
 
   Section FPlus.
     Definition option_t_mzero {A} : option_t m A := OptionT $ ret None.
