src/Structures/Category.v
@@ -1,6 +1,7 @@
 Require Import FP.Structures.Proxy.
 Require Import FP.Structures.Eqv.
-Require Import FP.Structures.EqvRel.
+Require Import FP.Structures.EqvEnv.
+Require Import FP.Structures.Feq.
 Require Import FP.Structures.EqDec.
 Require Import FP.Data.Function.
 Require Import FP.Relations.Setoid.
@@ -11,67 +12,57 @@ Class Category (t:Type -> Type -> Type) :=
   { cid : forall {A}, t A A
   ; ccompose : forall {A B C}, t B C -> t A B -> t A C
   }.
+Arguments cid {t Category A} : simpl never.
+Arguments ccompose {t Category A B C} _ _ : simpl never.
 
 Section CategoryWF.
   Context {t:Type->Type->Type}.
   Context {Category_:Category t}.
   Context {EqvEnv_:EqvEnv}.
-  Context {EqvEnvWF_:EqvEnvWF}.
-  Context {tPER:forall {A} {aER:PE_R A} {B} {bER:PE_R B}, PE_R (t A B)}.
+  Context {EqvEnvLogical_:EqvEnvLogical}.
+  Context {tPER :
+    forall
+      {A} {aER:Px (env_PER A)}
+      {B} {bER:Px (env_PER B)},
+    Px (env_PER (t A B))}.
+  Context {tPER' :
+    forall
+      {A} {aER:Px (env_PER A)} {aER':Px (env_PER_WF A)}
+      {B} {bER:Px (env_PER B)} {bER':Px (env_PER_WF B)},
+    Px (env_PER_WF (t A B))}.
 
   Class CategoryWF :=
     { category_left_unit :
         forall
-          {A} {aER:PE_R A}
-          {B} {bER:PE_R B}
-          (f:t A B) {fP:Proper PE_eqv f},
-            PE_eqv
+          {A} {aER:Px (env_PER A)} {aER':Px (env_PER_WF A)}
+          {B} {bER:Px (env_PER B)} {bER':Px (env_PER_WF B)}
+          (f:t A B) {fP:Proper env_eqv f},
+            env_eqv
             (ccompose cid f)
             f
     ; category_right_unit :
         forall
-          {A} {aER:E_R A}
-          {B} {bER:E_R B}
-          (f:t A B) {fP:Proper PE_eqv f},
-            PE_eqv
+          {A} {aER:Px (env_PER A)} {aER':Px (env_PER_WF A)}
+          {B} {bER:Px (env_PER B)} {bER':Px (env_PER_WF B)}
+          (f:t A B) {fP:Proper env_eqv f},
+            env_eqv
             (ccompose f cid)
             f
     ; category_associativity :
         forall
-          {A} {aER:E_R A}
-          {B} {bER:E_R B}
-          {C} {cER:E_R C}
-          {D} {dER:E_R D}
-          (f:t A B) {fP:Proper PE_eqv f}
-          (g:t B C) {gP:Proper PE_eqv g}
-          (h:t C D) {hP:Proper PE_eqv h},
-            PE_eqv
+          {A} {aER:Px (env_PER A)} {aER':Px (env_PER_WF A)}
+          {B} {bER:Px (env_PER B)} {bER':Px (env_PER_WF B)}
+          {C} {cER:Px (env_PER C)} {cER':Px (env_PER_WF C)}
+          {D} {dER:Px (env_PER D)} {dER':Px (env_PER_WF D)}
+          (f:t A B) {fP:Proper env_eqv f}
+          (g:t B C) {gP:Proper env_eqv g}
+          (h:t C D) {hP:Proper env_eqv h},
+            env_eqv
             (ccompose (ccompose h g) f)
             (ccompose h (ccompose g f))
     }.
 End CategoryWF.
-Arguments CategoryWF t {_ _ _ _}.
-
-Section CategoryWF_Eq.
-  Local Instance eqv_env : EqvEnv := eq_EqvEnv.
-  Local Instance eqv_env_wf : EqvEnvWF := eq_EqvEnvWF.
-  Context {t:Type->Type->Type}.
-  Context {Category:Category t}.
-  Context {CategoryWF:CategoryWF t (EqvEnv_:=eq_EqvEnv)}.
-  Definition category_right_unit_eq
-    {A B} (f:t A B) : eq (ccompose f cid) f :=
-      category_right_unit f f (reflexivity f).
-  Definition category_left_unit_eq
-    {A} {B} (f:t A B) : eq (ccompose cid f) f :=
-      category_left_unit f f (reflexivity f).
-  Definition category_associativity_eq
-    {A} {B} {C} {D} (f:t A B) (g:t B C) (h:t C D) :
-      eq (ccompose (ccompose h g) f) (ccompose h (ccompose g f)) :=
-    category_associativity
-      f f (reflexivity f)
-      g g (reflexivity g)
-      h h (reflexivity h).
-End CategoryWF_Eq.
+Arguments CategoryWF t {_ _ _}.
 
 Module CategoryNotation.
   Infix "<.>" := ccompose (at level 45, right associativity).
