src/Structures/Deriving.v
@@ -5,6 +5,7 @@ Require Import FP.Structures.Eqv.
 Require Import FP.Structures.Injection.
 Require Import FP.Structures.Lattice.
 Require Import FP.Structures.Ord.
+Require Import FP.Structures.EqvEnv.
 Require Import FP.Relations.Setoid.
 
 Import FunctionNotation.
@@ -48,19 +49,17 @@ Section DerivingInjResp_inv.
   Variable (to:T -> U).
   Variable (from:U -> T).
   Variable (TR:T -> T -> Prop) (UR:U -> U -> Prop).
+  Context {PER_TR:PER TR}.
   Context {InjResp2:InjectionRespect U T from UR TR}.
-  Variable (eqv:T -> T -> Prop).
-  Context {Eqv:Equivalence eqv}.
-  Context {InjInv:InjectionInverse T U to from eqv}.
-  Context {TR_Resp:Proper (eqv ==> eqv ==> impl) TR}.
+  Context {InjInv:InjectionInverse T U to from eq}.
   Variable (poof:UR = (TR `on` from)).
 
   Definition DerivingInjResp_inv : InjectionRespect T U to TR UR.
   Proof. constructor ; unfold Proper,"==>","<==" ; simpl ; intros.
     rewrite poof ; simpl.
-      repeat rewrite <- InjectionInverse_inv ; auto.
+      repeat erewrite <- InjectionInverse_inv ; auto.
     rewrite poof in H ; simpl in H.
-      repeat rewrite <- InjectionInverse_inv in H ; auto.
+      repeat erewrite <- InjectionInverse_inv in H ; auto.
   Qed.
 End DerivingInjResp_inv.
 
@@ -112,7 +111,8 @@ Section DerivingInjectionDistribute_ext.
   Context {P:Proper (eqv1 ==> eqv1 ==> impl) eqv2}.
 
   Definition DerivingInjectionDistribute_ext : InjectionDistribute T U to TM UM eqv2.
-  Proof. constructor ; intros.
+  Proof.
+    constructor ; intros.
     rewrite InjectionDistribute_law.
     reflexivity.
   Qed.
@@ -126,7 +126,8 @@ Section DerivingEqRDC.
   Variable (poof:(eq_dec (T:=T)) = (eq_dec `on` inj)).
 
   Definition DerivingEqRDC : RelDecCorrect T eq eq_dec.
-  Proof. repeat (constructor ; simpl in * ; intros).
+  Proof.
+    repeat (constructor ; simpl in * ; intros).
     rewrite poof ; simpl.
       apply rel_correct.
       apply InjectionRespect_eta ; auto.
@@ -136,13 +137,31 @@ Section DerivingEqRDC.
     Qed.
 End DerivingEqRDC.
 
-Section DerivingEqvWF.
-  Context {T} {T_Eqv:Eqv T} {U} {U_Eqv:Eqv U} {U_EqvWF:EqvWF U}.
+Section DerivingEqv_PE_WF.
+  Context {T} {T_Eqv:Eqv T} {U} {U_Eqv:Eqv U} {U_EqvWF:Eqv_PE_WF U}.
   Variable (inj:T -> U).
   Context {T_U_InjResp:InjectionRespect T U inj eqv eqv}.
 
-  Definition DerivingEqvWF : EqvWF T.
-  Proof. repeat constructor.
+  Definition DerivingEqv_PE_WF : Eqv_PE_WF T.
+  Proof.
+    repeat constructor.
+    unfold Symmetric ; intros.
+      apply InjectionRespect_beta ; apply InjectionRespect_eta in H ; symmetry ; auto.
+    unfold Transitive ; intros x y z H1 H2.
+      apply InjectionRespect_beta.
+      apply InjectionRespect_eta in H1 ; apply InjectionRespect_eta in H2.
+      transitivity (inj y) ; auto.
+  Qed.
+End DerivingEqv_PE_WF.
+
+Section DerivingEqv_E_WF.
+  Context {T} {T_Eqv:Eqv T} {U} {U_Eqv:Eqv U} {U_EqvWF:Eqv_E_WF U}.
+  Variable (inj:T -> U).
+  Context {T_U_InjResp:InjectionRespect T U inj eqv eqv}.
+
+  Definition DerivingEqv_E_WF : Eqv_E_WF T.
+  Proof.
+    repeat constructor.
     unfold Reflexive ; intros.
       apply InjectionRespect_beta ; reflexivity.
     unfold Symmetric ; intros.
@@ -152,11 +171,11 @@ Section DerivingEqvWF.
       apply InjectionRespect_eta in H1 ; apply InjectionRespect_eta in H2.
       transitivity (inj y) ; auto.
   Qed.
-End DerivingEqvWF.
+End DerivingEqv_E_WF.
 
 Section DerivingOrdWF.
-  Context {T} {T_Eqv:Eqv T} {T_EqvWF:EqvWF T} {T_Ord:Ord T}.
-  Context {U} {U_Eqv:Eqv U} {U_EqvWF:EqvWF U} {U_Ord:Ord U} {U_OrdWF:OrdWF U}.
+  Context {T} {T_Eqv:Eqv T} {T_EqvWF:Eqv_E_WF T} {T_Ord:Ord T}.
+  Context {U} {U_Eqv:Eqv U} {U_EqvWF:Eqv_E_WF U} {U_Ord:Ord U} {U_OrdWF:OrdWF U}.
   Variable (inj:T -> U).
   Context {InjResp_eqv:InjectionRespect T U inj eqv eqv}.
   Context {InjResp_lt:InjectionRespect T U inj lt lt}.
@@ -209,11 +228,11 @@ End DerivingOrdDecCorrect.
 
 Section DerivingLatticeWF.
   Context {T:Type}.
-  Context {T_Eqv:Eqv T} {T_EqvWF:EqvWF T}.
+  Context {T_Eqv:Eqv T} {T_EqvWF:Eqv_E_WF T}.
   Context {T_Ord:Ord T} {T_OrdWF:OrdWF T}.
   Context {T_Lattice:Lattice T}.
   Context {U:Type}.
-  Context {U_Eqv:Eqv U} {U_EqvWF:EqvWF U}.
+  Context {U_Eqv:Eqv U} {U_EqvWF:Eqv_E_WF U}.
   Context {U_Ord:Ord U} {U_OrdWF:OrdWF U}.
   Context {U_Lattice:Lattice U} {U_LatticeWF:LatticeWF U}.
   Variable (inj:T -> U).
@@ -234,12 +253,12 @@ End DerivingLatticeWF.
 
 Section DerivingBoundedLatticeWF.
   Context {T:Type}.
-  Context {T_Eqv:Eqv T} {T_EqvWF:EqvWF T}.
+  Context {T_Eqv:Eqv T} {T_EqvWF:Eqv_E_WF T}.
   Context {T_Ord:Ord T} {T_OrdWF:OrdWF T}.
   Context {T_Lattice:Lattice T}.
   Context {T_BoundedLattice:BoundedLattice T}.
   Context {U:Type}.
-  Context {U_Eqv:Eqv U} {U_EqvWF:EqvWF U}.
+  Context {U_Eqv:Eqv U} {U_EqvWF:Eqv_E_WF U}.
   Context {U_Ord:Ord U} {U_OrdWF:OrdWF U}.
   Context {U_Lattice:Lattice U}.
   Context {U_BoundedLattice:BoundedLattice U} {U_BoundedLatticeWF:BoundedLatticeWF U}.
@@ -268,84 +287,600 @@ Module Type DerivingTheKitchenSink1_Arg.
   Parameter U : Type -> Type.
   Parameter to : forall {A}, T A -> U A.
   Parameter from : forall {A}, U A -> T A.
-  Parameter InjResp : forall A, InjectionRespect (T A) (U A) to eq eq.
-  Parameter InjInv : forall A, InjectionInverse (U A) (T A) from to eq.
+  Parameter InjResp : forall {A}, InjectionRespect (T A) (U A) to eq eq.
+  Parameter InjInv : forall {A}, InjectionInverse (U A) (T A) from to eq.
+  Global Declare Instance U_EqDec :
+    forall {A} {EqDec_:EqDec A},
+    EqDec (U A).
+  Global Declare Instance U_EqDec_RDC :
+    forall {A} {EqDec_:EqDec A} {RDC_A:RelDecCorrect A eq eq_dec},
+    RelDecCorrect (U A) eq eq_dec.
+  Global Declare Instance U_Eqv :
+    forall {A} {Eqv_:Eqv A},
+    Eqv (U A).
+  Global Declare Instance U_Eqv_PE_WF :
+    forall {A} {Eqv_:Eqv A} {Eqv_PE_WF_:Eqv_PE_WF A},
+    Eqv_PE_WF (U A).
+  Global Declare Instance U_Eqv_E_WF :
+    forall {A} {Eqv_:Eqv A} {Eqv_E_WF_:Eqv_E_WF A},
+    Eqv_E_WF (U A).
+  Global Declare Instance U_EqvDec :
+    forall {A} {EqvDec_:EqvDec A},
+    EqvDec (U A).
+  Global Declare Instance U_EqvDec_RDC :
+    forall {A} {Eqv_:Eqv A} {EqvDec_:EqvDec A} {RDC_A:RelDecCorrect A eqv eqv_dec},
+    RelDecCorrect (U A) eqv eqv_dec.
+  Global Declare Instance U_Ord :
+    forall {A} {Ord_:Ord A},
+    Ord (U A).
+  Global Declare Instance U_OrdWF :
+    forall {A}
+      {Eqv_:Eqv A} {Eqv_E_WF_:Eqv_E_WF A}
+      {Ord_:Ord A} {Ord_WF_:OrdWF A},
+    OrdWF (U A).
+  Global Declare Instance U_OrdDec :
+    forall {A} {OrdDec_:OrdDec A},
+    OrdDec (U A).
+  Global Declare Instance U_ODC :
+    forall {A}
+        {Eqv_:Eqv A}
+        {Ord_:Ord A} {OrdDec_:OrdDec A} {ODC_A:OrdDecCorrect A},
+    OrdDecCorrect (U A).
+  Global Declare Instance U_Lattice :
+    forall {A} {Lattice_:Lattice A},
+    Lattice (U A).
+  Global Declare Instance U_LatticeWF :
+    forall {A}
+      {Eqv_:Eqv A} {Eqv_E_WF_:Eqv_E_WF A}
+      {Ord_:Ord A} {OrdWF_:OrdWF A}
+      {Lattice_:Lattice A} {LatticeWF_:LatticeWF A},
+    LatticeWF (U A).
+  Global Declare Instance U_BoundedLattice :
+    forall {A} {BoundedLattice_:BoundedLattice A},
+    BoundedLattice (U A).
+  Global Declare Instance U_BoundedLatticeWF :
+    forall {A}
+      {Eqv_:Eqv A} {Eqv_E_WF_:Eqv_E_WF A}
+      {Ord_:Ord A} {OrdWF_:OrdWF A}
+      {Lattice_:Lattice A} {LatticeWF_:LatticeWF A}
+      {BoundedLattice_:BoundedLattice A} {BoundedLatticeWF_:BoundedLatticeWF A},
+    BoundedLatticeWF (U A).
 End DerivingTheKitchenSink1_Arg.
 
 Module DerivingTheKitchenSink1 (X:DerivingTheKitchenSink1_Arg).
   Import X.
+  Arguments T _ /.
+  Arguments U _ /.
   Arguments to {A} _ /.
   Arguments from {A} _ /.
 
   Section Context.
     Context {A:Type}.
-    Context {U_EqDec:EqDec (U A)} {U_RDC_eq:RelDecCorrect (U A) eq eq_dec}.
-    Context {U_Eqv:Eqv (U A)} {U_EqvWF:EqvWF (U A)}.
-    Context {U_EqvDec:EqvDec (U A)} {U_RDC_eqv:RelDecCorrect (U A) eqv eqv_dec}.
-    Context {U_Ord:Ord (U A)} {U_OrdWF:OrdWF (U A)}.
-    Context {U_OrdDec:OrdDec (U A)} {U_ODC:OrdDecCorrect (U A)}.
-    Context {U_Lattice:Lattice (U A)} {U_LatticeWF:LatticeWF (U A)}.
-    Context {U_BLattice:BoundedLattice (U A)} {U_BLatticeWF:BoundedLatticeWF (U A)}.
 
-    Global Instance DTKS_EqDec : EqDec (T A) := { eq_dec := eq_dec `on` to }.
-    Global Instance DTKS_EqDec_RDC : RelDecCorrect (T A) eq eq_dec :=
-      DerivingEqRDC to eq_refl.
+    Section EqDec.
+      Context {EqDec_:EqDec A} {EqDec_RDC_:RelDecCorrect A eq eq_dec}.
 
-    Global Instance DTKS_Eqv : Eqv (T A) := { eqv := eqv `on` to }.
-    Global Instance DTKS_InjectionRespect_to_eqv
-        : InjectionRespect (T A) (U A) to eqv eqv :=
-      DerivingInjResp to eqv eqv eq_refl.
-    Global Instance DTKS_InjectionRespect_from_eqv
-        : InjectionRespect (U A) (T A) from eqv eqv :=
-      DerivingInjResp_inv from to eqv eqv eq eq_refl.
-    Global Instance DTKS_EqvWF : EqvWF (T A) :=
-      DerivingEqvWF to.
-    Global Instance DTKS_InjectionInverse_from_eqv
-        : InjectionInverse (U A) (T A) from to eqv :=
-      DerivingInjectionInverse_ext from to eq eqv.
+      Global Instance DTKS_EqDec : EqDec (T A) := { eq_dec := eq_dec `on` to }.
+      Global Instance DTKS_EqDec_RDC : RelDecCorrect (T A) eq eq_dec :=
+        DerivingEqRDC to eq_refl.
+    End EqDec.
 
-    Global Instance DTKS_EqvDec : EqvDec (T A) := { eqv_dec := eqv_dec `on` to }.
-    Global Instance DTKS_EqvDec_RDC : RelDecCorrect (T A) eqv eqv_dec :=
-      DerivingRelDec to eqv eqv_dec eqv eqv_dec eq_refl.
+    Section Eqv.
+      Context {Eqv_:Eqv A}.
 
-    Global Instance DTKS_Ord : Ord (T A) := { lt := lt `on` to }.
-    Global Instance DTKS_InjectionRespect_to_lt
-        : InjectionRespect (T A) (U A) to lt lt :=
-      DerivingInjResp to lt lt eq_refl.
-    Global Instance DTKS_InjectionRespect_from_lt
-        : InjectionRespect (U A) (T A) from lt lt :=
-      DerivingInjResp_inv from to lt lt eq eq_refl.
-    Global Instance DTKS_OrdWF : OrdWF (T A) :=
-      DerivingOrdWF to.
+      Global Instance DTKS_Eqv : Eqv (T A) := { eqv := eqv `on` to }.
+      Global Instance DTKS_InjectionRespect_to_eqv
+          : InjectionRespect (T A) (U A) to eqv eqv :=
+        DerivingInjResp to eqv eqv eq_refl.
+    End Eqv.
 
-    Global Instance DTKS_OrdDec : OrdDec (T A) := { ord_dec := ord_dec `on` to }.
-    Global Instance DTKS_ODC : OrdDecCorrect (T A) :=
-      DerivingOrdDecCorrect to eq_refl.
+    Section Eqv_PE_WF.
+      Context {Eqv_:Eqv A} {Eqv_PE_WF_:Eqv_PE_WF A}.
 
-    Global Instance DTKS_Lattice : Lattice (T A) :=
-      { lmeet := from '..' (lmeet `on` to)
-      ; ljoin := from '..' (ljoin `on` to)
-      }.
-    Global Instance DTKS_InjectionDistribute_lmeet_eq
-        : InjectionDistribute (T A) (U A) to lmeet lmeet eq :=
-      DerivingInjectionDistribute to from lmeet lmeet eq eq_refl.
-    Global Instance DTKS_InjectionDistribute_lmeet_eqv
-        : InjectionDistribute (T A) (U A) to lmeet lmeet eqv :=
-      DerivingInjectionDistribute_ext to lmeet lmeet eq eqv.
-    Global Instance DTKS_InjectionDistribute_ljoin_eq
-        : InjectionDistribute (T A) (U A) to ljoin ljoin eq :=
-      DerivingInjectionDistribute to from ljoin ljoin eq eq_refl.
-    Global Instance DTKS_InjectionDistribute_ljoin_eqv
-        : InjectionDistribute (T A) (U A) to ljoin ljoin eqv :=
-      DerivingInjectionDistribute_ext to ljoin ljoin eq eqv.
-    Global Instance DTKS_LatticeWF : LatticeWF (T A) :=
-      DerivingLatticeWF to.
+      Global Instance DTKS_Eqv_PE_WF : Eqv_PE_WF (T A) :=
+        DerivingEqv_PE_WF to.
+      Global Instance DTKS_PE_InjectionRespect_from_eqv
+          : InjectionRespect (U A) (T A) from eqv eqv :=
+        DerivingInjResp_inv from to eqv eqv eq_refl.
+    End Eqv_PE_WF.
 
-    Global Instance DTKS_BoundedLattice : BoundedLattice (T A) :=
-      { ltop := from ltop
-      ; lbot := from lbot
-      }.
-    Global Instance DTKS_BoundedLatticeWF : BoundedLatticeWF (T A) :=
-      DerivingBoundedLatticeWF to from eq_refl eq_refl.
+    Section Eqv_E_WF.
+      Context {Eqv_:Eqv A} {Eqv_E_WF_:Eqv_E_WF A}.
+
+      Global Instance DTKS_Eqv_E_WF : Eqv_E_WF (T A) :=
+        DerivingEqv_E_WF to.
+      Global Instance DTKS_E_InjectionRespect_from_eqv
+          : InjectionRespect (U A) (T A) from eqv eqv :=
+        DerivingInjResp_inv from to eqv eqv eq_refl.
+      Global Instance DTKS_InjectionInverse_from_eqv
+          : InjectionInverse (U A) (T A) from to eqv :=
+        DerivingInjectionInverse_ext from to eq eqv.
+    End Eqv_E_WF.
+
+    Section EqvDec.
+      Context {Eqv_:Eqv A} {EqvDec_:EqvDec A} {EqvDec_RDC_:RelDecCorrect A eqv eqv_dec}.
+
+      Global Instance DTKS_EqvDec : EqvDec (T A) := { eqv_dec := eqv_dec `on` to }.
+      Global Instance DTKS_EqvDec_RDC : RelDecCorrect (T A) eqv eqv_dec :=
+        DerivingRelDec to eqv eqv_dec eqv eqv_dec eq_refl.
+    End EqvDec.
+
+    Section Ord.
+      Context {Eqv_:Eqv A} {Eqv_PE_WF_:Eqv_E_WF A} {Ord_:Ord A} {OrdWF_:OrdWF A}.
+      Context {OrdDec_:OrdDec A} {ODC_:OrdDecCorrect A}.
+
+      Global Instance DTKS_Ord : Ord (T A) := { lt := lt `on` to }.
+      Global Instance DTKS_InjectionRespect_to_lt
+          : InjectionRespect (T A) (U A) to lt lt :=
+        DerivingInjResp to lt lt eq_refl.
+      Global Instance DTKS_InjectionRespect_from_lt
+          : InjectionRespect (U A) (T A) from lt lt :=
+        DerivingInjResp_inv from to lt lt eq_refl.
+      Global Instance DTKS_OrdWF : OrdWF (T A) :=
+        DerivingOrdWF to.
+
+      Global Instance DTKS_OrdDec : OrdDec (T A) := { ord_dec := ord_dec `on` to }.
+      Global Instance DTKS_ODC : OrdDecCorrect (T A) :=
+        DerivingOrdDecCorrect to eq_refl.
+    End Ord.
+
+    Section Lattice.
+      Context {Eqv_:Eqv A} {EqvWF_:Eqv_E_WF A}.
+      Context {Ord_:Ord A} {OrdWF_:OrdWF A}.
+      Context {Lattice_:Lattice A} {LatticeWF_:LatticeWF A}.
+      Context {BLattice_:BoundedLattice A} {BLatticeWF_:BoundedLatticeWF A}.
+
+      Global Instance DTKS_Lattice : Lattice (T A) :=
+        { lmeet := from '..' (lmeet `on` to)
+        ; ljoin := from '..' (ljoin `on` to)
+        }.
+      Global Instance DTKS_InjectionDistribute_lmeet_eq
+          : InjectionDistribute (T A) (U A) to lmeet lmeet eq :=
+        DerivingInjectionDistribute to from lmeet lmeet eq eq_refl.
+      Global Instance DTKS_InjectionDistribute_lmeet_eqv
+          : InjectionDistribute (T A) (U A) to lmeet lmeet eqv :=
+        DerivingInjectionDistribute_ext to lmeet lmeet eq eqv.
+      Global Instance DTKS_InjectionDistribute_ljoin_eq
+          : InjectionDistribute (T A) (U A) to ljoin ljoin eq :=
+        DerivingInjectionDistribute to from ljoin ljoin eq eq_refl.
+      Global Instance DTKS_InjectionDistribute_ljoin_eqv
+          : InjectionDistribute (T A) (U A) to ljoin ljoin eqv :=
+        DerivingInjectionDistribute_ext to ljoin ljoin eq eqv.
+      Global Instance DTKS_LatticeWF : LatticeWF (T A) :=
+        DerivingLatticeWF to.
+
+      Global Instance DTKS_BoundedLattice : BoundedLattice (T A) :=
+        { ltop := from ltop
+        ; lbot := from lbot
+        }.
+      Global Instance DTKS_BoundedLatticeWF : BoundedLatticeWF (T A) :=
+        DerivingBoundedLatticeWF to from eq_refl eq_refl.
+    End Lattice.
   End Context.
 End DerivingTheKitchenSink1.
+
+Class depend {T} (X:T) := {}.
+Instance : forall {T} {X:T}, depend X := {}.
+
+Module Type DerivingTheKitchenSink2_Arg.
+  Parameter T : (Type -> Type) -> Type -> Type.
+  Parameter U : (Type -> Type) -> Type -> Type.
+  Parameter to : forall {m A}, T m A -> U m A.
+  Parameter from : forall {m A}, U m A -> T m A.
+  Parameter InjResp : forall {m A}, InjectionRespect (T m A) (U m A) to eq eq.
+  Parameter InjInv : forall {m A}, InjectionInverse (U m A) (T m A) from to eq.
+  Section m.
+    Context {m:Type->Type}.
+    Global Declare Instance U_EqDec :
+      forall
+        {EqDec_m :
+           forall {X} {EqDec_:EqDec X},
+           EqDec (m X)}
+        {A} {EqDec_:EqDec A},
+      EqDec (U m A).
+    Global Declare Instance U_EqDec_RDC :
+      forall
+        {EqDec_m :
+           forall {X} {EqDec_:EqDec X},
+           EqDec (m X)}
+        {EqDec_RDC_m :
+           forall {X} {EqDec_:EqDec X} {EqDec_RDC_:RelDecCorrect X eq eq_dec},
+           RelDecCorrect (m X) eq eq_dec}
+        {A} {EqDec_:EqDec A} {RDC_A:RelDecCorrect A eq eq_dec},
+      RelDecCorrect (U m A) eq eq_dec.
+    Global Declare Instance U_Eqv :
+      forall
+        {Eqv_m :
+           forall {X} {Eqv_:Eqv X},
+           Eqv (m X)}
+        {A} {Eqv_:Eqv A},
+      Eqv (U m A).
+    Global Declare Instance U_Eqv_PE_WF :
+      forall
+        {Eqv_m :
+           forall {X} {Eqv_:Eqv X},
+           Eqv (m X)}
+        {Eqv_PE_WF_m :
+           forall {X} {Eqv_:Eqv X} {Eqv_PE_WF_:Eqv_PE_WF X},
+           Eqv_PE_WF (m X)}
+        {A} {Eqv_:Eqv A} {Eqv_PE_WF_:Eqv_PE_WF A},
+      Eqv_PE_WF (U m A).
+    Global Declare Instance U_Eqv_E_WF :
+      forall
+        {Eqv_m :
+           forall {X} {Eqv_:Eqv X},
+           Eqv (m X)}
+        {Eqv_E_WF_m :
+           forall {X} {Eqv_:Eqv X} {Eqv_E_WF_:Eqv_E_WF X},
+           Eqv_E_WF (m X)}
+        {A} {Eqv_:Eqv A} {Eqv_E_WF_:Eqv_E_WF A},
+      Eqv_E_WF (U m A).
+    Global Declare Instance U_EqvDec :
+      forall
+        {EqvDec_m :
+           forall {X} {EqvDec_:EqvDec X},
+            EqvDec (m X)}
+        {A} {EqvDec_:EqvDec A},
+      EqvDec (U m A).
+    Global Declare Instance U_EqvDec_RDC :
+      forall
+        {Eqv_m :
+           forall {X} {Eqv_:Eqv X},
+           Eqv (m X)}
+        {EqvDec_m :
+           forall {X} {EqvDec_:EqvDec X},
+           EqvDec (m X)}
+        {EqvDec_RDC_m :
+           forall
+             {X} {Eqv_:Eqv X} {EqvDec_:EqvDec X}
+             {RDC_A:RelDecCorrect X eqv eqv_dec},
+           RelDecCorrect (m X) eqv eqv_dec}
+        {A} {Eqv_:Eqv A} {EqvDec_:EqvDec A} {RDC_A:RelDecCorrect A eqv eqv_dec},
+      RelDecCorrect (U m A) eqv eqv_dec.
+    Global Declare Instance U_Ord :
+      forall
+        {Ord_m :
+           forall {X} {Ord_:Ord X},
+           Ord (m X)}
+        {A} {Ord_:Ord A},
+      Ord (U m A).
+    Global Declare Instance U_OrdWF :
+      forall
+        {Eqv_m :
+           forall {X} {Eqv_:Eqv X},
+           Eqv (m X)}
+        {Eqv_E_WF_m :
+           forall {X} {Eqv_:Eqv X} {Eqv_E_WF_:Eqv_E_WF X},
+           Eqv_E_WF (m X)}
+        {Ord_m :
+           forall {X} {Ord_:Ord X},
+           Ord (m X)}
+        {OrdWF_m :
+           forall
+             {X}
+             {Eqv_:Eqv X} {Eqv_E_WF_:Eqv_E_WF X}
+             {Ord_:Ord X} {Ord_WF_:OrdWF X},
+           OrdWF (m X)}
+        {A}
+        {Eqv_:Eqv A} {Eqv_E_WF_:Eqv_E_WF A}
+        {Ord_:Ord A} {Ord_WF_:OrdWF A},
+      OrdWF (U m A).
+    Global Declare Instance U_OrdDec :
+      forall
+        {OrdDec_m :
+           forall {X} {OrdDec_:OrdDec X},
+           OrdDec (m X)}
+        {A} {OrdDec_:OrdDec A},
+      OrdDec (U m A).
+    Global Declare Instance U_ODC :
+      forall
+        {Eqv_m :
+           forall {X} {Eqv_:Eqv X},
+           Eqv (m X)}
+        {Ord_m :
+           forall {X} {Ord_:Ord X},
+           Ord (m X)}
+        {OrdDec_m :
+           forall {X} {OrdDec_:OrdDec X},
+           OrdDec (m X)}
+        {ODC_m :
+           forall
+             {X} {Eqv_:Eqv X}
+             {Ord_:Ord X} {OrdDec_:OrdDec X} {ODC_A:OrdDecCorrect X},
+           OrdDecCorrect (m X)}
+        {A}
+        {Eqv_:Eqv A}
+        {Ord_:Ord A} {OrdDec_:OrdDec A} {ODC_A:OrdDecCorrect A},
+      OrdDecCorrect (U m A).
+    Global Declare Instance U_Lattice :
+      forall
+        {Lattice_m :
+           forall {X} {Lattice_:Lattice X},
+           Lattice (m X)}
+        {A} {Lattice_:Lattice A},
+      Lattice (U m A).
+    Global Declare Instance U_LatticeWF :
+      forall
+        {Eqv_m :
+           forall {X} {Eqv_:Eqv X},
+           Eqv (m X)}
+        {Eqv_E_WF_m :
+           forall {X} {Eqv_:Eqv X} {Eqv_E_WF_:Eqv_E_WF X},
+           Eqv_E_WF (m X)}
+        {Ord_m :
+           forall {X} {Ord_:Ord X},
+           Ord (m X)}
+        {OrdWF_m :
+           forall
+             {X}
+             {Eqv_:Eqv X} {Eqv_E_WF_:Eqv_E_WF X}
+             {Ord_:Ord X} {Ord_WF_:OrdWF X},
+           OrdWF (m X)}
+        {Lattice_m :
+           forall {X} {Lattice_:Lattice X},
+           Lattice (m X)}
+        {LatticeWF_m :
+           forall {X}
+             {Eqv_:Eqv X} {Eqv_E_WF_:Eqv_E_WF X}
+             {Ord_:Ord X} {OrdWF_:OrdWF X}
+             {Lattice_:Lattice X} {LatticeWF_:LatticeWF X},
+           LatticeWF (m X)}
+        {A}
+        {Eqv_:Eqv A} {Eqv_E_WF_:Eqv_E_WF A}
+        {Ord_:Ord A} {OrdWF_:OrdWF A}
+        {Lattice_:Lattice A} {LatticeWF_:LatticeWF A},
+      LatticeWF (U m A).
+    Global Declare Instance U_BoundedLattice :
+      forall 
+        {BoundedLattice_m :
+           forall {X} {BoundedLattice_:BoundedLattice X},
+           BoundedLattice (m X)}
+        {A} {BoundedLattice_:BoundedLattice A},
+      BoundedLattice (U m A).
+    Global Declare Instance U_BoundedLatticeWF :
+      forall
+        {Eqv_m :
+           forall {X} {Eqv_:Eqv X},
+           Eqv (m X)}
+        {Eqv_E_WF_m :
+           forall {X} {Eqv_:Eqv X} {Eqv_E_WF_:Eqv_E_WF X},
+           Eqv_E_WF (m X)}
+        {Ord_m :
+           forall {X} {Ord_:Ord X},
+           Ord (m X)}
+        {OrdWF_m :
+           forall
+             {X}
+             {Eqv_:Eqv X} {Eqv_E_WF_:Eqv_E_WF X}
+             {Ord_:Ord X} {Ord_WF_:OrdWF X},
+           OrdWF (m X)}
+        {Lattice_m :
+           forall {X} {Lattice_:Lattice X},
+           Lattice (m X)}
+        {LatticeWF_m :
+           forall {X}
+             {Eqv_:Eqv X} {Eqv_E_WF_:Eqv_E_WF X}
+             {Ord_:Ord X} {OrdWF_:OrdWF X}
+             {Lattice_:Lattice X} {LatticeWF_:LatticeWF X},
+           LatticeWF (m X)}
+        {BoundedLattice_m :
+           forall {X} {BoundedLattice_:BoundedLattice X},
+           BoundedLattice (m X)}
+        {BoundedLatticeWF_m :
+           forall {X}
+             {Eqv_:Eqv X} {Eqv_E_WF_:Eqv_E_WF X}
+             {Ord_:Ord X} {OrdWF_:OrdWF X}
+             {Lattice_:Lattice X} {LatticeWF_:LatticeWF X}
+             {BoundedLattice_:BoundedLattice X} {BoundedLatticeWF_:BoundedLatticeWF X},
+           BoundedLatticeWF (m X)}
+        {A}
+        {Eqv_:Eqv A} {Eqv_E_WF_:Eqv_E_WF A}
+        {Ord_:Ord A} {OrdWF_:OrdWF A}
+        {Lattice_:Lattice A} {LatticeWF_:LatticeWF A}
+        {BoundedLattice_:BoundedLattice A} {BoundedLatticeWF_:BoundedLatticeWF A},
+      BoundedLatticeWF (U m A).
+  End m.
+End DerivingTheKitchenSink2_Arg.
+
+Module DerivingTheKitchenSink2 (X:DerivingTheKitchenSink2_Arg).
+  Import X.
+  Arguments T _ _ /.
+  Arguments U _ _ /.
+  Arguments to {m A} _ /.
+  Arguments from {m A} _ /.
+
+  Section Context.
+    Context {m:Type->Type} {A:Type}.
+
+    Section EqDec.
+      Context {EqDec_:EqDec A} {EqDec_RDC_:RelDecCorrect A eq eq_dec}.
+      Context {EqDec_m :
+        forall {X} {EqDec_:EqDec X},
+        EqDec (m X)}.
+      Context {EqDec_RDC_m :
+        forall {X} {EqDec_:EqDec X} {EqDec_RDC_:RelDecCorrect X eq eq_dec},
+        RelDecCorrect (m X) eq eq_dec}.
+
+      Global Instance DTKS_EqDec : EqDec (T m A) := { eq_dec := eq_dec `on` to }.
+      Global Instance DTKS_EqDec_RDC : RelDecCorrect (T m A) eq eq_dec :=
+        DerivingEqRDC to eq_refl.
+    End EqDec.
+
+    Section Eqv.
+      Context {Eqv_:Eqv A}.
+      Context {Eqv_m :
+        forall {X} {Eqv_:Eqv X},
+        Eqv (m X)}.
+
+      Global Instance DTKS_Eqv : Eqv (T m A) := { eqv := eqv `on` to }.
+      Global Instance DTKS_InjectionRespect_to_eqv
+          : InjectionRespect (T m A) (U m A) to eqv eqv :=
+        DerivingInjResp to eqv eqv eq_refl.
+    End Eqv.
+
+    Section Eqv_PE_WF.
+      Context {Eqv_:Eqv A} {EqvWF_:Eqv_PE_WF A}.
+      Context {Eqv_m :
+        forall {X} {Eqv_:Eqv X},
+        Eqv (m X)}.
+      Context {Eqv_PE_WF_m :
+        forall {X} {Eqv_:Eqv X} {Eqv_PE_WF_:Eqv_PE_WF X},
+        Eqv_PE_WF (m X)}.
+
+      Global Instance DTKS_PE_EqvWF : Eqv_PE_WF (T m A) :=
+        DerivingEqv_PE_WF to.
+      Global Instance DTKS_PE_InjectionRespect_from_eqv
+          : InjectionRespect (U m A) (T m A) from eqv eqv :=
+        DerivingInjResp_inv from to eqv eqv eq_refl.
+    End Eqv_PE_WF.
+
+    Section Eqv_E_WF.
+      Context {Eqv_:Eqv A} {EqvWF_:Eqv_E_WF A}.
+      Context {Eqv_m :
+        forall {X} {Eqv_:Eqv X},
+        Eqv (m X)}.
+      Context {Eqv_E_WF_m :
+        forall {X} {Eqv_:Eqv X} {Eqv_E_WF_:Eqv_E_WF X},
+        Eqv_E_WF (m X)}.
+
+      Global Instance DTKS_E_EqvWF : Eqv_E_WF (T m A) :=
+        DerivingEqv_E_WF to.
+      Global Instance DTKS_E_InjectionRespect_from_eqv
+          : InjectionRespect (U m A) (T m A) from eqv eqv :=
+        DerivingInjResp_inv from to eqv eqv eq_refl.
+      Global Instance DTKS_InjectionInverse_from_eqv
+          : InjectionInverse (U m A) (T m A) from to eqv :=
+        DerivingInjectionInverse_ext from to eq eqv.
+    End Eqv_E_WF.
+
+    Section EqvDec.
+      Context {Eqv_:Eqv A} {EqvDec_:EqvDec A}.
+      Context {EqvDec_RDC_:RelDecCorrect A eqv eqv_dec}.
+      Context {Eqv_m :
+        forall {X} {Eqv_:Eqv X},
+        Eqv (m X)}.
+      Context {EqvDec_m :
+        forall {X} {EqvDec_:EqvDec X},
+        EqvDec (m X)}.
+      Context {EqvDec_RDC_m :
+        forall
+          {X} {Eqv_:Eqv X} {EqvDec_:EqvDec X}
+          {RDC_A:RelDecCorrect X eqv eqv_dec},
+        RelDecCorrect (m X) eqv eqv_dec}.
+
+      Global Instance DTKS_EqvDec : EqvDec (T m A) := { eqv_dec := eqv_dec `on` to }.
+      Global Instance DTKS_EqvDec_RDC : RelDecCorrect (T m A) eqv eqv_dec :=
+        DerivingRelDec to eqv eqv_dec eqv eqv_dec eq_refl.
+    End EqvDec.
+
+    Section Ord.
+      Context {Eqv_:Eqv A} {EqvWF_:Eqv_E_WF A}.
+      Context {Ord_:Ord A} {OrdWF_:OrdWF A}.
+      Context {OrdDec_:OrdDec A} {ODC_:OrdDecCorrect A}.
+      Context {Eqv_m :
+        forall {X} {Eqv_:Eqv X},
+        Eqv (m X)}.
+      Context {Eqv_E_WF_m :
+        forall {X} {Eqv_:Eqv X} {Eqv_E_WF_:Eqv_E_WF X},
+        Eqv_E_WF (m X)}.
+      Context {Ord_m :
+        forall {X} {Ord_:Ord X},
+        Ord (m X)}.
+      Context {OrdWF_m :
+        forall
+          {X}
+          {Eqv_:Eqv X} {Eqv_E_WF_:Eqv_E_WF X}
+          {Ord_:Ord X} {Ord_WF_:OrdWF X},
+        OrdWF (m X)}.
+      Context {OrdDec_m :
+        forall {X} {OrdDec_:OrdDec X},
+        OrdDec (m X)}.
+      Context {ODC_m :
+        forall
+          {X} {Eqv_:Eqv X}
+          {Ord_:Ord X} {OrdDec_:OrdDec X} {ODC_A:OrdDecCorrect X},
+        OrdDecCorrect (m X)}.
+
+      Global Instance DTKS_Ord : Ord (T m A) := { lt := lt `on` to }.
+      Global Instance DTKS_InjectionRespect_to_lt
+          : InjectionRespect (T m A) (U m A) to lt lt :=
+        DerivingInjResp to lt lt eq_refl.
+      Global Instance DTKS_InjectionRespect_from_lt
+          : InjectionRespect (U m A) (T m A) from lt lt :=
+        DerivingInjResp_inv from to lt lt eq_refl.
+      Global Instance DTKS_OrdWF : OrdWF (T m A) :=
+        DerivingOrdWF to.
+
+      Global Instance DTKS_OrdDec : OrdDec (T m A) := { ord_dec := ord_dec `on` to }.
+      Global Instance DTKS_ODC : OrdDecCorrect (T m A) :=
+        DerivingOrdDecCorrect to eq_refl.
+    End Ord.
+
+    Section Lattice.
+      Context {Eqv_:Eqv A} {EqvWF_:Eqv_E_WF A}.
+      Context {Ord_:Ord A} {OrdWF_:OrdWF A}.
+      Context {Lattice_:Lattice A} {LatticeWF_:LatticeWF A}.
+      Context {BLattice_:BoundedLattice A} {BLatticeWF_:BoundedLatticeWF A}.
+      Context {Eqv_m :
+        forall {X} {Eqv_:Eqv X},
+        Eqv (m X)}.
+      Context {Eqv_E_WF_m :
+        forall {X} {Eqv_:Eqv X} {Eqv_E_WF_:Eqv_E_WF X},
+        Eqv_E_WF (m X)}.
+      Context {Ord_m :
+        forall {X} {Ord_:Ord X},
+        Ord (m X)}.
+      Context {OrdWF_m :
+        forall
+          {X}
+          {Eqv_:Eqv X} {Eqv_E_WF_:Eqv_E_WF X}
+          {Ord_:Ord X} {Ord_WF_:OrdWF X},
+        OrdWF (m X)}.
+      Context {Lattice_m :
+        forall {X} {Lattice_:Lattice X},
+        Lattice (m X)}.
+      Context {LatticeWF_m :
+        forall {X}
+          {Eqv_:Eqv X} {Eqv_E_WF_:Eqv_E_WF X}
+          {Ord_:Ord X} {OrdWF_:OrdWF X}
+          {Lattice_:Lattice X} {LatticeWF_:LatticeWF X},
+        LatticeWF (m X)}.
+      Context {BoundedLattice_m :
+        forall {X} {BoundedLattice_:BoundedLattice X},
+        BoundedLattice (m X)}.
+      Context {BoundedLatticeWF_m :
+        forall {X}
+          {Eqv_:Eqv X} {Eqv_E_WF_:Eqv_E_WF X}
+          {Ord_:Ord X} {OrdWF_:OrdWF X}
+          {Lattice_:Lattice X} {LatticeWF_:LatticeWF X}
+          {BoundedLattice_:BoundedLattice X} {BoundedLatticeWF_:BoundedLatticeWF X},
+        BoundedLatticeWF (m X)}.
+
+      Global Instance DTKS_Lattice : Lattice (T m A) :=
+        { lmeet := from '..' (lmeet `on` to)
+        ; ljoin := from '..' (ljoin `on` to)
+        }.
+      Global Instance DTKS_InjectionDistribute_lmeet_eq
+          : InjectionDistribute (T m A) (U m A) to lmeet lmeet eq :=
+        DerivingInjectionDistribute to from lmeet lmeet eq eq_refl.
+      Global Instance DTKS_InjectionDistribute_lmeet_eqv
+          : InjectionDistribute (T m A) (U m A) to lmeet lmeet eqv :=
+        DerivingInjectionDistribute_ext to lmeet lmeet eq eqv.
+      Global Instance DTKS_InjectionDistribute_ljoin_eq
+          : InjectionDistribute (T m A) (U m A) to ljoin ljoin eq :=
+        DerivingInjectionDistribute to from ljoin ljoin eq eq_refl.
+      Global Instance DTKS_InjectionDistribute_ljoin_eqv
+          : InjectionDistribute (T m A) (U m A) to ljoin ljoin eqv :=
+        DerivingInjectionDistribute_ext to ljoin ljoin eq eqv.
+      Global Instance DTKS_LatticeWF : LatticeWF (T m A) :=
+        DerivingLatticeWF to.
+
+      Global Instance DTKS_BoundedLattice : BoundedLattice (T m A) :=
+        { ltop := from ltop
+        ; lbot := from lbot
+        }.
+      Global Instance DTKS_BoundedLatticeWF : BoundedLatticeWF (T m A) :=
+        DerivingBoundedLatticeWF to from eq_refl eq_refl.
+    End Lattice.
+  End Context.
+End DerivingTheKitchenSink2.
