src/Structures/Eqv.v
@@ -1,19 +1,21 @@
 Require Import FP.Data.Function.
 Require Import FP.Relations.RelDec.
 Require Import FP.Structures.Injection.
-Require Import FP.Structures.EqvRel.
+Require Import FP.Structures.EqvEnv.
 Require Import FP.Structures.Proxy.
 Require Import FP.Relations.Setoid.
 
 Import FunctionNotation.
+Import ProperNotation.
 
 Class Eqv T := { eqv : T -> T -> Prop }.
+
 Arguments eqv {T Eqv} _ _ : simpl never.
 
-Definition Eqv_Proxy2 {T} {Eqv_:Eqv T} : Proxy (Eqv T) := {| proxy := Eqv_ |}.
-Definition Proxy2_Eqv {T} {Proxy2_:Proxy (Eqv T)} : Eqv T := proxy Proxy2_.
-Hint Resolve Eqv_Proxy2 : typeclass_instances.
-Hint Immediate Proxy2_Eqv : typeclass_instances.
+Definition Eqv_Px {T} {Eqv_:Eqv T} : Px (Eqv T) := Eqv_.
+Definition Px_Eqv {T} {Px_:Px (Eqv T)} : Eqv T := Px_.
+Hint Resolve Eqv_Px : typeclass_instances.
+Hint Immediate Px_Eqv : typeclass_instances.
 
 Section Eqv.
   Context {T} {Eqv_:Eqv T}.
@@ -21,8 +23,148 @@ Section Eqv.
   Definition not_eqv : T -> T -> Prop := not '..' eqv.
 End Eqv.
 
-Class EqvWF T {Eqv_:Eqv T} := { eqv_equivalence :> Equivalence eqv }.
-Class PEqvWF T {Eqv_:Eqv T} := { peqv_equivalence :> PER eqv }.
+Class Eqv_E_WF T {Eqv_:Eqv T} := { eqv_E_WF :> Equivalence eqv }.
+Class Eqv_PE_WF T {Eqv_:Eqv T} := { eqv_PE_WF :> PER eqv }.
+
+Definition Eqv_PE_WF_Px {T} {Eqv_:Eqv T} {Eqv_PE_WF_:Eqv_PE_WF T}
+    : Px (Eqv_PE_WF T) := Eqv_PE_WF_.
+Definition Px_Eqv_PE_WF {T} {Eqv_:Px (Eqv T)} {Px_:Px (Eqv_PE_WF T)}
+    : Eqv_PE_WF T := Px_.
+Hint Resolve Eqv_PE_WF_Px : typeclass_instances.
+Hint Immediate Px_Eqv_PE_WF : typeclass_instances.
+
+Definition eqv_EqvEnv : EqvEnv :=
+  {| env_PER := Eqv
+  ;  env_eqv := fun T (p:Px (Eqv T)) => eqv
+  ;  env_PER_WF := fun T (p:Px (Eqv T)) => Eqv_PE_WF T
+  ;  env_eqv_WF := fun T (p:Px (Eqv T)) (pwf:Px (Eqv_PE_WF T)) => eqv_PE_WF
+  |}.
+Section EqvEnv.
+  Local Instance EqvEnv_ : EqvEnv := eqv_EqvEnv.
+  Global Instance env_eqv_WF_eqv {T} {p:Eqv T} {pwf:Eqv_PE_WF T} : PER env_eqv.
+  Proof.
+    pose (@env_eqv_WF _ T).
+    auto.
+  Qed.
+End EqvEnv.
+
+Section Fun_Eqv.
+  Context {A} {aF:Eqv A} {B} {bF:Eqv B}.
+  Local Instance Fun_Eqv : Eqv (A -> B) :=
+    { eqv := (eqv ==> eqv) }.
+
+  Variable (aPEWF:Eqv_PE_WF A) (bPEWF:Eqv_PE_WF B).
+  Local Instance Fun_Eqv_PE_WF : Eqv_PE_WF (A -> B).
+  Proof.
+    inversion aPEWF ; inversion bPEWF.
+    repeat econstructor.
+    - unfold Symmetric ; eapply symmetry.
+    - unfold Transitive ; eapply transitivity.
+  Qed.
+End Fun_Eqv.
+
+Section Eqv_EqvEnvLogical.
+  Local Instance EqvEnv2_ : EqvEnv := eqv_EqvEnv.
+  Definition eqv_EqvEnvLogical : EqvEnvLogical.
+  Proof.
+    econstructor ; intros.
+    apply Fun_Eqv_PE_WF ; auto.
+    simpl ; auto.
+    simpl in H ; auto.
+  Qed.
+End Eqv_EqvEnvLogical.
+
+Section EqvEnvLogical.
+  Local Instance EqvEnv3_ : EqvEnv := eqv_EqvEnv.
+  Local Instance EqvEnvLogical_ : EqvEnvLogical := eqv_EqvEnvLogical.
+  Global Instance eqv_env_logical_P_eqv :
+    forall
+      {A} {aP:Eqv A}
+      {B} {bP:Eqv B},
+    Eqv (A -> B).
+  Proof.
+    intros.
+    pose (@eqv_env_logical_P _ _ A _ B _).
+    auto.
+  Defined.
+  Global Instance eqv_env_logical_PE_WF :
+    forall
+      {A} {aP:Eqv A} {aPWF:Eqv_PE_WF A}
+      {B} {bP:Eqv B} {bPWF:Eqv_PE_WF B},
+    Eqv_PE_WF (A -> B).
+  Proof.
+    intros.
+    assert (Px (Eqv_PE_WF A)) ; eauto with typeclass_instances.
+    assert (Px (Eqv_PE_WF B)) ; eauto with typeclass_instances.
+    pose (@eqv_env_logical_PE_WF _ _ A _ _ B _ _).
+    auto.
+  Qed.
+  Definition eqv_env_logical_intro_eqv :
+    forall
+      {A} {aP:Eqv A}
+      {B} {bP:Eqv B}
+      {f:A -> B} {g:A -> B},
+    (eqv ==> eqv) f g -> eqv f g.
+  Proof.
+    intros.
+    pose (@eqv_env_logical_intro _ _).
+    unfold env_eqv in e ; simpl in e.
+    eauto.
+  Qed.
+  Definition eqv_env_logical_elim_eqv :
+    forall
+      {A} {aP:Eqv A}
+      {B} {bP:Eqv B}
+      {f:A -> B} {g:A -> B},
+    eqv f g -> (eqv ==> eqv) f g.
+  Proof.
+    intros.
+    pose (@eqv_env_logical_elim _ _).
+    eauto.
+  Qed.
+End EqvEnvLogical.
+
+Ltac logical_eqv_intro_once_eqv :=
+  match goal with
+  | [ |- eqv ?A ?B ] =>
+      match type of A with
+      | ?T -> ?U => apply eqv_env_logical_intro_eqv ; unfold "==>" at 1 ; intros
+      | Fun ?T ?U => apply eqv_env_logical_intro_eqv ; unfold "==>" at 1 ; intros
+      end
+  end.
+
+Ltac logical_eqv_intro_eqv := repeat logical_eqv_intro_once_eqv.
+Ltac logical_eqv_elim_once_eqv :=
+  match goal with
+  | [ |- eqv (?f ?x) (?g ?y) ] => apply eqv_env_logical_elim_eqv
+  end.
+Ltac logical_eqv_elim_eqv := repeat logical_eqv_elim_once_eqv.
+
+Create HintDb logical_eqv_db_eqv.
+
+Ltac logical_eqv_once_eqv :=
+  match goal with
+  | [ |- eqv (?f ?x) (?g ?y) ] =>
+      let g_type := type of g in
+      match type of f with
+      | g_type => logical_eqv_elim_once_eqv
+      end
+  | [ |- eqv (fun _ => _) _ ] =>
+      logical_eqv_intro_once_eqv
+  | [ |- eqv _ (fun _ => _) ] =>
+      logical_eqv_intro_once_eqv
+  end.
+Ltac logical_eqv_eqv :=
+  match goal with
+  | [ |- Proper eqv ?x ] => unfold Proper
+  | _ => idtac
+  end ;
+  repeat logical_eqv_once_eqv ;
+  match goal with
+  | [ |- eqv ?x ?x ] => change (eqv x x) with (Proper eqv x)
+  | _ => idtac
+  end ;
+  eauto with logical_eqv_db_eqv typeclass_instances.
 
 Class EqvDec T := { eqv_dec : T -> T -> bool }.
 Section EqvDec.
@@ -38,25 +180,6 @@ Section EqvDec.
   Definition neg_eqv_dec_p : forall x y:T, {~eqv x y} + {eqv x y} := neg_rel_dec_p.
 End EqvDec.
 Arguments eqv_dec {T EqvDec} _ _ : simpl never.
-
-Definition eqv_EqvEnv : EqvEnv :=
-  {| eqv_env_eqv_P := Eqv
-  ;  eqv_env_eqv := fun T (Proxy2_:Proxy2 Eqv T) => eqv
-  ;  eqv_env_E_PWF := fun T (p:Proxy2 Eqv T) => EqvWF T
-  ;  eqv_env_E_WF := fun T (p:Proxy2 Eqv T) (pwf:EqvWF T) => eqv_equivalence
-  ;  eqv_env_PE_PWF := fun T (p:Proxy2 Eqv T) => PEqvWF T
-  ;  eqv_env_PE_WF := fun T (p:Proxy2 Eqv T) (pwf:PEqvWF T) => peqv_equivalence
-  |}.
-Instance eqv_E_R {A} {Eqv_:Eqv A} {EqvWF_:EqvWF A} :
-    E_R (EqvEnv_:=eqv_EqvEnv) A :=
-  { E_R_eqv_P := Eqv_Proxy2
-  ; E_R_eqv_PWF := EqvWF_ 
-  }.
-Instance eqv_PE_R {A} {PEqv_:Eqv A} {PEqvWF_:PEqvWF A} :
-    PE_R (EqvEnv_:=eqv_EqvEnv) A :=
-  { PE_R_eqv_P := Eqv_Proxy2
-  ; PE_R_eqv_PWF := PEqvWF_ 
-  }.
 
 Module EqvNotation.
   Infix "~=!" := eqv_dec (at level 35, no associativity).
