src/Structures/EqvEnv.v
@@ -1,3 +1,4 @@
+Require Import FP.Data.Function.
 Require Import FP.Structures.Proxy.
 Require Import FP.Relations.Setoid.
 
@@ -5,97 +6,99 @@ Import ProperNotation.
 
 Class EqvEnv :=
   { (* equivalence *)
-    eqv_env_eqv_P : Type -> Type
-  ; eqv_env_eqv : forall {T} {p:Proxy (eqv_env_eqv_P T)}, T -> T -> Prop
+    env_PER : Type -> Type
+  ; env_eqv : forall {T} {p:Px (env_PER T)}, T -> T -> Prop
   ; (* eqv is a partial equivalence relation *)
-    eqv_env_PE_PWF : forall (T:Type) {p:Proxy (eqv_env_eqv_P T)}, Type
-  ; eqv_env_PE_WF :
-      forall {T} {p:Proxy (eqv_env_eqv_P T)} {pwf:Proxy (eqv_env_PE_PWF T)},
-        PER eqv_env_eqv
+    env_PER_WF : forall (T:Type) {p:Px (env_PER T)}, Type
+  ; env_eqv_WF :>
+      forall {T} {p:Px (env_PER T)} {pwf:Px (env_PER_WF T)},
+      PER env_eqv
   }.
+Arguments env_eqv {EqvEnv T p} _ _ : simpl never.
 
-Class EqvEnvWF {EqvEnv_:EqvEnv} :=
-  { eqv_env_functional_eqv_P :>
+Class EqvEnvLogical {EqvEnv_:EqvEnv} :=
+  { eqv_env_logical_P :>
       forall
-        {A} {aP:Proxy (eqv_env_eqv_P A)}
-        {B} {bP:Proxy (eqv_env_eqv_P B)},
-          Proxy (eqv_env_eqv_P (A -> B))
-  ; eqv_env_functional_PE_PWF :
+        {A} {aP:Px (env_PER A)}
+        {B} {bP:Px (env_PER B)},
+      Px (env_PER (A -> B))
+  ; eqv_env_logical_PE_WF :>
       forall
-        {A} {aP:Proxy (eqv_env_eqv_P A)} (aPWF:Proxy (eqv_env_PE_PWF A))
-        {B} {bP:Proxy (eqv_env_eqv_P B)} (bPWF:Proxy (eqv_env_PE_PWF B)),
-          Proxy (eqv_env_PE_PWF (A -> B))
+        {A} {aP:Px (env_PER A)} (aPWF:Px (env_PER_WF A))
+        {B} {bP:Px (env_PER B)} (bPWF:Px (env_PER_WF B)),
+      Px (env_PER_WF (A -> B))
   ; eqv_env_logical_intro :
       forall
-        {A} {aPER:Proxy (eqv_env_eqv_P A)}
-        {B} {bPER:Proxy (eqv_env_eqv_P B)}
+        {A} {aPER:Px (env_PER A)}
+        {B} {bPER:Px (env_PER B)}
         {f:A -> B} {g:A -> B},
-          (eqv_env_eqv ==> eqv_env_eqv) f g -> eqv_env_eqv f g
+      (env_eqv ==> env_eqv) f g -> env_eqv f g
   ; eqv_env_logical_elim :
       forall
-        {A} {aPER:Proxy (eqv_env_eqv_P A)}
-        {B} {bPER:Proxy (eqv_env_eqv_P B)}
+        {A} {aPER:Px (env_PER A)}
+        {B} {bPER:Px (env_PER B)}
         {f:A -> B} {g:A -> B},
-          eqv_env_eqv f g -> (eqv_env_eqv ==> eqv_env_eqv) f g
+      env_eqv f g -> (env_eqv ==> env_eqv) f g
   }.
 
-Section PE_R.
+(*
+not sure if this is needed or not
+Section EqvEnv.
   Context {EqvEnv_:EqvEnv}.
+  Context {EqvEnvLogical_:EqvEnvLogical}.
 
-  Class PE_R (T:Type) : Type :=
-    { PE_R_eqv_P :> Proxy (eqv_env_eqv_P T)
-    ; PE_R_eqv_PWF : Proxy (eqv_env_PE_PWF T)
-    }.
+  Global Instance eqv_env_logical_P' :
+    forall
+      {P}
+      {A} {aP:Px (P A)}
+      {B} {bP:Px (P B)}
+      (e:P = env_PER),
+    Px (P (A -> B)).
+  Proof.
+    intros.
+    rewrite e in *.
+    eauto with typeclass_instances.
+  Qed.
+End EqvEnv.
+*)
 
-  Context {T} {PE_R_:PE_R T}.
-  Definition PE_eqv : T -> T -> Prop := eqv_env_eqv.
-  Global Instance PE_R_env_peqv_WF : PER eqv_env_eqv :=
-    eqv_env_PE_WF (pwf:=PE_R_eqv_PWF).
-End PE_R.
-
-Section EqvEnvWF.
+Section EqvEnvLogical.
   Context {EqvEnv_:EqvEnv}.
-  Context {EqvEnvWF_:EqvEnvWF}.
-
-  Section Fun_PE_R.
-    Context {A} {aER:PE_R A}.
-    Context {B} {bER:PE_R B}.
-    Global Instance EqvEnvWF_Fun_E_R : PE_R (A -> B) :=
-      {| PE_R_eqv_P := eqv_env_functional_eqv_P
-       ; PE_R_eqv_PWF := eqv_env_functional_PE_PWF PE_R_eqv_PWF PE_R_eqv_PWF
-      |}.
-  End Fun_PE_R.
+  Context {EqvEnvWF_:EqvEnvLogical}.
 
   Section Proper_Elim.
-    Context {A} {aER:PE_R A}.
-    Context {B} {aBR:PE_R B}.
-    Context {f:A -> B} {fP:Proper PE_eqv f}.
-    Global Instance Proper_PE_R_elim1 : Proper (PE_eqv ==> PE_eqv) f :=
+    Context {A} {aER:Px (env_PER A)} {aER':Px (env_PER_WF A)}.
+    Context {B} {bER:Px (env_PER B)} {bER':Px (env_PER_WF B)}.
+    Context {f:A -> B} {fP:Proper env_eqv f}.
+    Global Instance Proper_PE_R_elim1 : Proper (env_eqv ==> env_eqv) f :=
       eqv_env_logical_elim fP.
 
-    Context {C} {cER:PE_R C} {g:A -> B -> C} {gP:Proper PE_eqv g}.
-    Global Instance Proper_PE_R_elim2 : Proper (PE_eqv ==> PE_eqv ==> PE_eqv) g.
+    Context {C} {cER:Px (env_PER C)} {cER':Px (env_PER_WF C)}.
+    Context {g:A -> B -> C} {gP:Proper env_eqv g}.
+    Global Instance Proper_PE_R_elim2 : Proper (env_eqv ==> env_eqv ==> env_eqv) g.
       unfold Proper,"==>" at 1 ; intros.
       repeat apply eqv_env_logical_elim ; auto.
     Qed.
   End Proper_Elim.
 
   Section Proper_App.
-    Context {A} {aER:PE_R A}.
-    Context {B} {aBR:PE_R B}.
-    Context {x:A} {xP:Proper PE_eqv x}.
-    Context {f:A -> B} {fP:Proper PE_eqv f}.
-    Global Instance Proper_PE_R_app : Proper PE_eqv (f x) := Proper_PE_R_elim1 x x xP.
+    Context {A} {aER:Px (env_PER A)} {aER':Px (env_PER_WF A)}.
+    Context {B} {bER:Px (env_PER B)} {bER':Px (env_PER_WF B)}.
+    Context (x:A) {xP:Proper env_eqv x}.
+    Context (f:A -> B) {fP:Proper env_eqv f}.
+    Global Instance Proper_PE_R_app : Proper env_eqv (f x) := Proper_PE_R_elim1 x x xP.
   End Proper_App.
-End EqvEnvWF.
+End EqvEnvLogical.
 
 Ltac logical_eqv_intro_once :=
   match goal with
   | [ |- ?R ?A ?B ] =>
       match type of A with
       | ?T -> ?U => apply eqv_env_logical_intro ; unfold "==>" at 1 ; intros
+      | Fun ?T ?U => apply eqv_env_logical_intro ; unfold "==>" at 1 ; intros
       end
   end.
+
 Ltac logical_eqv_intro := repeat logical_eqv_intro_once.
 Ltac logical_eqv_elim_once :=
   match goal with
@@ -104,3 +107,48 @@ Ltac logical_eqv_elim_once :=
 Ltac logical_eqv_elim := repeat logical_eqv_elim_once.
 
 Create HintDb logical_eqv_db.
+
+Ltac logical_eqv_once :=
+  match goal with
+  | [ |- env_eqv (?f ?x) (?g ?y) ] =>
+      let g_type := type of g in
+      match type of f with
+      | g_type => logical_eqv_elim_once
+      end
+  | [ |- env_eqv (fun _ => _) _ ] =>
+      logical_eqv_intro_once
+  | [ |- env_eqv _ (fun _ => _) ] =>
+      logical_eqv_intro_once
+  end.
+Ltac logical_eqv :=
+  match goal with
+  | [ |- Proper env_eqv ?x ] => unfold Proper
+  | _ => idtac
+  end ;
+  repeat logical_eqv_once ;
+  match goal with
+  | [ |- env_eqv ?x ?x ] => change (env_eqv x x) with (Proper env_eqv x)
+  | _ => idtac
+  end ;
+  eauto with logical_eqv_db typeclass_instances.
+     
+Section morph_proper.
+  Context {EqvEnv_:EqvEnv}.
+  Context {T:Type} {tPER:Px (env_PER T)} {tPER_WF:Px (env_PER_WF T)}.
+  Context {x:T} {y:T}.
+  Context (fP:env_eqv x y).
+  Definition morph_proper_left : Proper env_eqv x.
+  Proof.
+    unfold Proper.
+    transitivity y ; auto.
+    symmetry ; auto.
+  Qed.
+  Definition morph_proper_right : Proper env_eqv y.
+  Proof.
+    unfold Proper.
+    transitivity x ; auto.
+    symmetry ; auto.
+  Qed.
+End morph_proper.
+Hint Resolve morph_proper_left : logical_eqv_db.
+Hint Resolve morph_proper_right : logical_eqv_db.
