src/Structures/FUnit.v
@@ -1,4 +1,6 @@
-Require Import FP.Structures.EqvRel.
+Require Import FP.Structures.EqvEnv.
+Require Import FP.Structures.Proxy.
+Require Import FP.Structures.Eqv.
 Require Import FP.Relations.Setoid.
 
 Import ProperNotation.
@@ -10,13 +12,38 @@ Section FUnitWF.
   Context {t:Type -> Type}.
   Context {FUnit_:FUnit t}.
   Context {EqvEnv_:EqvEnv}.
-  Context {EqvEnvWF_:EqvEnvWF}.
-  Context {E_R_t:forall {A} {aER:PE_R A}, PE_R (t A)}.
+  Context {EqvEnvLogical_:EqvEnvLogical}.
+  Context {E_R_t:forall {A} {aPE:Px (env_PER A)}, Px (env_PER (t A))}.
+  Context {E_R_WF_t :
+    forall {A} {aPE:Px (env_PER A)} {aPEWF:Px (env_PER_WF A)},
+    Px (env_PER_WF (t A))}.
 
   Class FUnitWF :=
     { funit_respect :>
-        forall {A} {aER:PE_R A},
-          Proper PE_eqv (funit (A:=A))
+        forall {A} {aER:Px (env_PER A)} {aER':Px (env_PER_WF A)},
+        Proper env_eqv (funit (A:=A))
     }.
 End FUnitWF.
 Arguments FUnitWF t {_ _ _ _}.
+Hint Extern 9 (Proper env_eqv funit) => apply funit_respect : typeclass_instances.
+
+Section EqvEnv_eqv.
+  Local Instance EqvEnv_ : EqvEnv := eqv_EqvEnv.
+  Local Instance EqvEnvLogical_ : EqvEnvLogical := eqv_EqvEnvLogical.
+  Context {t:Type -> Type}.
+  Context {FUnit_:FUnit t}.
+  Context {E_R_t:forall {A} {aPE:Eqv A}, Eqv (t A)}.
+  Context {E_R_WF_t :
+    forall {A} {aPE:Eqv A} {aPEWF:Eqv_PE_WF A},
+    Eqv_PE_WF (t A)}.
+  Context {FUnitWF_:FUnitWF t}.
+
+  Global Instance funit_respect_eqv :
+    forall {A} {aER:Eqv A} {aER':Eqv_PE_WF A},
+    Proper eqv (funit (A:=A)).
+  Proof.
+    intros.
+    pose (@funit_respect _ _ _ _ _).
+    eauto.
+  Qed.
+End EqvEnv_eqv.
