src/Structures/Feq.v
@@ -6,61 +6,39 @@ Import ProperNotation.
 
 Class Feq T :=
   { feq : T -> T -> Prop }.
-Definition Feq_Proxy2 {T} {Feq_:Feq T} : Proxy (Feq T) := {| proxy := Feq_ |}.
-Definition Proxy2_Feq {T} {Feq_:Proxy (Feq T)} : Feq T := proxy Feq_.
-Hint Resolve Feq_Proxy2 : typeclass_instances.
-Hint Immediate Proxy2_Feq : typeclass_instances.
+Definition Feq_Px {T} {Feq_:Feq T} : Px (Feq T) := Feq_.
+Definition Px_Feq {T} {Px_:Px (Feq T)} : Feq T := Px_.
+Hint Resolve Feq_Px : typeclass_instances.
+Hint Immediate Px_Feq : typeclass_instances.
 
 Class Feq_E_WF T {Feq_:Feq T} :=
   { feq_E_WF : Equivalence feq }.
 Class Feq_PE_WF T {Feq_:Feq T} :=
   { feq_PE_WF : PER feq }.
+Definition Feq_PE_WF_Px {T} {Feq_:Feq T} {Feq_PE_WF_:Feq_PE_WF T}
+    : Px (Feq_PE_WF T) := Feq_PE_WF_.
+Definition Px_Feq_PE_WF {T} {Feq_:Feq T} {Px_:Px (Feq_PE_WF T)}
+    : Feq_PE_WF T := Px_.
+Hint Resolve Feq_PE_WF_Px : typeclass_instances.
+Hint Immediate Px_Feq_PE_WF : typeclass_instances.
+
 Class FeqIsEq T {Feq_:Feq T} :=
   { feq_is_eq :  feq = eq }.
 
 Definition feq_EqvEnv : EqvEnv :=
-  {| eqv_env_eqv_P := @Feq
-  ;  eqv_env_eqv := fun T (p:Proxy2 Feq T) => feq
-  ;  eqv_env_E_PWF := fun T (p:Proxy2 Feq T) => Feq_E_WF T
-  ;  eqv_env_E_WF := fun T (p:Proxy2 Feq T) (pwf:Feq_E_WF T) => feq_E_WF
-  ;  eqv_env_PE_PWF := fun T (p:Proxy2 Feq T) => Feq_PE_WF T
-  ;  eqv_env_PE_WF := fun T (p:Proxy2 Feq T) (pwf:Feq_PE_WF T) => feq_PE_WF
+  {| env_PER := @Feq
+  ;  env_eqv := fun T (p:Px (Feq T)) => feq
+  ;  env_PER_WF := fun T (p:Px (Feq T)) => Feq_PE_WF T
+  ;  env_eqv_WF := fun T (p:Px (Feq T)) (pwf:Px (Feq_PE_WF T)) => feq_PE_WF
   |}.
-Section EqvEnvWF.
-  Context {EqvEnv_:EqvEnv}.
-  Class EqvEnvWF2 :=
-    { eqv_env_functional_eqv_P :>
-        forall
-          {A} {aP:Proxy2 eqv_env_eqv_P A}
-          {B} {bP:Proxy2 eqv_env_eqv_P B},
-            Proxy2 eqv_env_eqv_P (A -> B)
-    ; eqv_env_functional_PE_PWF :
-        forall
-          {A} {aP:Proxy2 eqv_env_eqv_P A} (aPWF:eqv_env_PE_PWF A)
-          {B} {bP:Proxy2 eqv_env_eqv_P B} (bPWF:eqv_env_PE_PWF B),
-            eqv_env_PE_PWF (A -> B)
-    ; eqv_env_logical_intro :
-        forall
-          {A} {aPER:Proxy2 eqv_env_eqv_P A}
-          {B} {bPER:Proxy2 eqv_env_eqv_P B}
-          {f:A -> B} {g:A -> B},
-            (eqv_env_eqv ==> eqv_env_eqv) f g -> eqv_env_eqv f g
-    ; eqv_env_logical_elim :
-        forall
-          {A} {aPER:Proxy2 eqv_env_eqv_P A}
-          {B} {bPER:Proxy2 eqv_env_eqv_P B}
-          {f:A -> B} {g:A -> B},
-            eqv_env_eqv f g -> (eqv_env_eqv ==> eqv_env_eqv) f g
-    }.
-End EqvEnvWF.
 
 Section Fun_Feq.
   Context {A} {aF:Feq A} {B} {bF:Feq B}.
-  Global Instance Fun_Feq : Feq (A -> B) | 2 :=
+  Global Instance Fun_Feq : Feq (A -> B) | 9 :=
     { feq := (feq ==> feq) }.
 
   Variable (aPEWF:Feq_PE_WF A) (bPEWF:Feq_PE_WF B).
-  Global Instance Fun_Feq_PE_WF : Feq_PE_WF (A -> B) | 2.
+  Global Instance Fun_Feq_PE_WF : Feq_PE_WF (A -> B) | 9.
   Proof.
     inversion aPEWF ; inversion bPEWF.
     repeat econstructor.
@@ -76,31 +54,20 @@ Section Fun_Feq.
 End Fun_Feq.
 Section Univ_Feq.
   Context {A:Type}.
-  Global Instance barf : Feq A | 3 :=
+  Local Instance Univ_Feq : Feq A | 10 :=
     { feq := eq }.
-  Global Instance bargl : Feq_PE_WF A | 3.
+  Local Instance Univ_Feq_PE_WF : Feq_PE_WF A | 10.
   Proof.
     repeat econstructor ; simpl ; auto ; unfold Transitive ; intros ; subst ; auto.
   Qed.
 End Univ_Feq.
 
-Print HintDb typeclass_instances.
-Section Fun_Feq2.
-  Global Instance foo : EqvEnvWF2 (EqvEnv_:=feq_EqvEnv).
+Section Feq_EqvEnvLogical.
+  Definition feq_EqvEnvLogical : EqvEnvLogical (EqvEnv_:=feq_EqvEnv).
   Proof.
     econstructor ; intros.
     apply Fun_Feq_PE_WF ; auto.
     simpl ; auto.
     simpl in H ; auto.
   Qed.
-End Fun_Feq2.
-
-Instance eq_E_R {A} : E_R (EqvEnv_:=eq_EqvEnv) A :=
-  { E_R_eqv_P := {| proxy2 := tt |}
-  ; E_R_eqv_PWF := tt
-  }.
-Instance eq_PE_R {A} : PE_R (EqvEnv_:=eq_EqvEnv) A :=
-  { PE_R_eqv_P := {| proxy2 := tt |}
-  ; PE_R_eqv_PWF := tt
-  }.
-                
+End Feq_EqvEnvLogical.
