src/Structures/Monad.v
@@ -1,5 +1,7 @@
 Require Import FP.Structures.FUnit.
-Require Import FP.Structures.EqvRel.
+Require Import FP.Structures.EqvEnv.
+Require Import FP.Structures.Proxy.
+Require Import FP.Structures.Eqv.
 Require Import FP.Relations.Setoid.
 Require Import FP.Data.Function.
 
@@ -30,11 +32,11 @@ Section Monad.
   Definition bind_mjoin {A} (aMM:m (m A)) : m A :=
     bind aMM id.
   Definition bind_fmap {A B} (f:A -> B) (aM:m A) : m B :=
-    bind aM (funit '.' f).
+    bind aM (ret '.' f).
   Definition bind_fapply {A B} (fM:m (A -> B)) (aM:m A) : m B :=
-    bind fM (fun f => bind aM (fun a => funit (f a))).
+    bind fM (fun f => bind aM (fun a => ret (f a))).
   Definition bind_ftimes {A B} (aM:m A) (bM:m B) : m (A*B) :=
-    bind aM (fun a => bind bM (fun b => funit (a,b))).
+    bind aM (fun a => bind bM (fun b => ret (a,b))).
 End Monad.
 Arguments ret {m FUnit_ A} _ /.
 Arguments extend {m MBind_ A B} _ _ /.
@@ -57,44 +59,117 @@ Module MonadNotation.
 End MonadNotation.
 
 Section MonadWF.
-  Variable (m:Type->Type).
+  Context {m:Type->Type}.
   Context {FUnit_:FUnit m} {MBind_:MBind m}.
   Context {EqvEnv_:EqvEnv}.
-  Context {EqvEnvWF_:EqvEnvWF}.
-  Context {E_R_m:forall {A} {aER:PE_R A}, PE_R (m A)}.
+  Context {EqvEnvLogical_:EqvEnvLogical}.
+  Context {PE_R_t:forall {A} {aER:Px (env_PER A)}, Px (env_PER (m A))}.
+  Context {PE_R_t' :
+    forall {A} {aER:Px (env_PER A)} {aER':Px (env_PER_WF A)},
+    Px (env_PER_WF (m A))}.
 
   Class MonadWF :=
     { bind_left_unit :
         forall
-          {A} {aER:E_R A}
-          {B} {bER:E_R B}
-          (f:A -> m B) {fP:Proper PE_eqv f}
-          (a:A) {aP:Proper PE_eqv a},
-            PE_eqv
-            (bind (ret a) f)
-            (f a)
+          {A} {aER:Px (env_PER A)} {aER':Px (env_PER_WF A)}
+          {B} {bER:Px (env_PER B)} {bER':Px (env_PER_WF B)}
+          (f:A -> m B) {fP:Proper env_eqv f}
+          (a:A) {aP:Proper env_eqv a},
+        env_eqv
+        (bind (ret a) f)
+        (f a)
     ; bind_right_unit :
         forall
-          {A} {aER:E_R A}
-          (aM:m A) {aMP:Proper PE_eqv aM},
-            PE_eqv
-            (bind aM ret)
-            aM
+          {A} {aER:Px (env_PER A)} {aER':Px (env_PER_WF A)}
+          (aM:m A) {aMP:Proper env_eqv aM},
+        env_eqv
+        (bind aM ret)
+        aM
     ; bind_associativity :
         forall
-          {A} {aER:E_R A}
-          {B} {bER:E_R B}
-          {C} {cER:E_R C}
-          (f:A -> m B) {fP:Proper PE_eqv f}
-          (g:B -> m C) {gP:Proper PE_eqv g}
-          (aM:m A) {aP:Proper PE_eqv aM},
-          PE_eqv
-          (bind (bind aM f) g)
-          (bind aM (fun a => bind (f a) g))
+          {A} {aER:Px (env_PER A)} {aER':Px (env_PER_WF A)}
+          {B} {bER:Px (env_PER B)} {bER':Px (env_PER_WF B)}
+          {C} {cER:Px (env_PER C)} {cER':Px (env_PER_WF C)}
+          (f:A -> m B) {fP:Proper env_eqv f}
+          (g:B -> m C) {gP:Proper env_eqv g}
+          (aM:m A) {aP:Proper env_eqv aM},
+        env_eqv
+        (bind (bind aM f) g)
+        (bind aM (fun a => bind (f a) g))
     ; bind_respect :>
         forall
-          {A} {aER:E_R A}
-          {B} {bER:E_R B},
-            Proper PE_eqv (bind (A:=A) (B:=B))
+          {A} {aER:Px (env_PER A)} {aER':Px (env_PER_WF A)}
+          {B} {bER:Px (env_PER B)} {bER':Px (env_PER_WF B)},
+        Proper env_eqv (bind (A:=A) (B:=B))
     }.
 End MonadWF.
+Arguments MonadWF m {_ _ _ _ _}.
+Hint Extern 9 (Proper env_eqv bind) => apply bind_respect : typeclass_instances.
+
+Section EqvEnv_eqv.
+  Local Instance EqvEnv_ : EqvEnv := eqv_EqvEnv.
+  Local Instance EqvEnvLogical_ : EqvEnvLogical := eqv_EqvEnvLogical.
+  Context {m:Type->Type}.
+  Context {FUnit_:FUnit m} {MBind_:MBind m}.
+  Context {PE_R_t:forall {A} {aER:Eqv A}, Eqv (m A)}.
+  Context {PE_R_t' :
+    forall {A} {aER:Eqv A} {aER':Eqv_PE_WF A},
+    Eqv_PE_WF (m A)}.
+  Context {MonadWF_:MonadWF m}.
+
+  Definition bind_left_unit_eqv :
+      forall
+        {A} {aER:Eqv A} {aER':Eqv_PE_WF A}
+        {B} {bER:Eqv B} {bER':Eqv_PE_WF B}
+        (f:A -> m B) {fP:Proper eqv f}
+        (a:A) {aP:Proper eqv a},
+      eqv
+      (bind (ret a) f)
+      (f a).
+  Proof.
+    intros.
+    pose (@bind_left_unit _ _ _ _ _ _ _).
+    eapply e ; auto.
+  Qed.
+
+  Definition bind_right_unit_eqv :
+    forall
+      {A} {aER:Eqv A} {aER':Eqv_PE_WF A}
+      (aM:m A) {aMP:Proper eqv aM},
+    eqv
+    (bind aM ret)
+    aM.
+  Proof.
+    intros.
+    pose (@bind_right_unit _ _ _ _ _ _ _).
+    eapply e ; auto.
+  Qed.
+
+  Definition bind_associativity_eqv :
+    forall
+      {A} {aER:Eqv A} {aER':Eqv_PE_WF A}
+      {B} {bER:Eqv B} {bER':Eqv_PE_WF B}
+      {C} {cER:Eqv C} {cER':Eqv_PE_WF C}
+      (f:A -> m B) {fP:Proper eqv f}
+      (g:B -> m C) {gP:Proper eqv g}
+      (aM:m A) {aP:Proper eqv aM},
+    eqv
+    (bind (bind aM f) g)
+    (bind aM (fun a => bind (f a) g)).
+  Proof.
+    intros.
+    pose (@bind_associativity _ _ _ _ _ _ _).
+    eapply e ; auto.
+  Qed.
+
+  Global Instance bind_respect_eqv :
+    forall
+      {A} {aER:Eqv A} {aER':Eqv_PE_WF A}
+      {B} {bER:Eqv B} {bER':Eqv_PE_WF B},
+    Proper eqv (bind (A:=A) (B:=B)).
+  Proof.
+    intros.
+    pose (@bind_respect _ _ _ _ _ _ _).
+    eapply p ; auto.
+  Qed.
+End EqvEnv_eqv.
