src/Data/Pretty.v
@@ -51,8 +51,6 @@ Inductive fmode :=
   | Flat
   | Break.
 
-Axiom undefined : forall {A}, A.
-
 Definition fits : Z -> list (N*fmode*doc) -> fuel bool :=
   mfix2 $ fun fits w ps =>
     if w <! 0%Z then
