src/Structures/FunctorP.v
@@ -1,4 +1,4 @@
 Require Import FP.Structures.Proxy.
 
 Class FMapP (P:Type->Type) (t:Type->Type) : Type :=
-  { fmap_p : forall {A B} {p:Proxy2 P B}, (A -> B) -> t A -> t B }.
+  { fmap_p : forall {A B} {p:Px (P B)}, (A -> B) -> t A -> t B }.
