src/Structures/MonadError.v
@@ -2,7 +2,7 @@ Require Import FP.Data.Function.
 Require Import FP.Data.String.
 Require Import FP.Structures.Injection.
 Require Import FP.Structures.Proxy.
-Require Import FP.Structures.EqvRel.
+Require Import FP.Structures.EqvEnv.
 Require Import FP.Structures.Monad.
 Require Import FP.Relations.Setoid.
 
@@ -29,45 +29,50 @@ Section MonadErrorWF.
   Context (E:Type) (m:Type->Type).
   Context {Monad_:Monad m} {MError_:MError E m}.
   Context {EqvEnv_:EqvEnv}.
-  Context {EqvEnvWF_:EqvEnvWF}.
-  Context {E_R_E:E_R E}.
-  Context {E_R_m:forall {A} {aER:E_R A}, E_R (m A)}.
+  Context {EqvEnvLogical_:EqvEnvLogical}.
+  Context {PE_R_E:Px (env_PER E)}.
+  Context {PE_R_E':Px (env_PER_WF E)}.
+  Context {PE_R_t:forall {A} {aER:Px (env_PER A)}, Px (env_PER (m A))}.
+  Context {PE_R_t' :
+    forall {A} {aER:Px (env_PER A)} {aER':Px (env_PER_WF A)},
+    Px (env_PER_WF (m A))}.
+
 
   Class MonadErrorWF :=
     { throw_left_zero :
         forall
-          {A} {aER:E_R A}
-          {B} {bER:E_R B}
-          (e:E) (e':E) (eP:E_eqv e e')
+          {A} {aER:Px (env_PER A)} {aER':Px (env_PER_WF A)}
+          {B} {bER:Px (env_PER B)} {bER':Px (env_PER_WF B)}
+          (e:E) (eP:Proper env_eqv e)
           (k:A -> m B),
-            E_eqv
+            env_eqv
             (bind (throw e) k)
-            (throw e')
+            (throw e)
     ; catch_of_throw :
         forall
-          {A} {aER:E_R A}
-          (e:E) (e':E) (eER:E_eqv e e')
-          (f:E -> m A) (f':E -> m A) (fP:PE_eqv f f'),
-            E_eqv
+          {A} {aER:Px (env_PER A)} {aER':Px (env_PER_WF A)}
+          (e:E) (eER:Proper env_eqv e)
+          (f:E -> m A) (fP:Proper env_eqv f),
+            env_eqv
             (catch (throw e) f)
-            (f' e)
+            (f e)
     ; catch_of_return :
         forall
-          {A} {aER:E_R A}
-          (a:A) (a':A) (aP:E_eqv a a')
+          {A} {aER:Px (env_PER A)} {aER':Px (env_PER_WF A)}
+          (a:A) (aP:Proper env_eqv a)
           (f:E -> m A),
-            E_eqv
+            env_eqv
             (catch (ret a) f)
-            (ret a')
+            (ret a)
     ; catch_associativity :
         forall
-          {A} {aER:E_R A}
-          (aM:m A) (aM':m A) (aMP:E_eqv aM aM')
-          (f:E -> m A) (f':E -> m A) (fP:PE_eqv f f')
-          (g:E -> m A) (g':E -> m A) (gP:PE_eqv g g'),
-            E_eqv
+          {A} {aER:Px (env_PER A)} {aER':Px (env_PER_WF A)}
+          (aM:m A) (aMP:Proper env_eqv aM)
+          (f:E -> m A) (fP:Proper env_eqv f)
+          (g:E -> m A) (gP:Proper env_eqv g),
+            env_eqv
             (catch (catch aM f) g)
-            (catch aM' (fun a => catch (f' a) g'))
+            (catch aM (fun a => catch (f a) g))
     }.
 End MonadErrorWF.
 
