loc.sh
@@ -1,0 +1,3 @@
+#!/bin/sh
+
+find -E . **/*.v | grep .v$ | xargs cat | wc -l 
