src/Structures/Proxy.v
@@ -1,7 +1,3 @@
 
-Class Proxy (P:Type) := { proxy : P }.
-Arguments proxy {P} Proxy.
-Class Proxy2 (P:Type->Type) (T:Type) : Type := { proxy2 : P T }.
-Arguments proxy2 {P T} Proxy2.
-Class Proxy3 (P:Type->Type->Type) (T:Type) (U:Type) : Type := { proxy3 : P T U }.
-Arguments proxy3 {P T U} Proxy3.
+Class Px (P:Type) := px : P.
+Arguments px {P} Px.
